IMP language; Coq certified equational reasoning based on the decorated logic.

Axioms.v
@@ -1,10 +1,11 @@
+
 (**************************************************************************)
-(*  This is part of IMP-STATES, it is distributed under the terms of the  *)
-(*              GNU Lesser General Public License version 3               *)
-(*                  (see file LICENSE for more details)                   *)
+(*  This is part of STATES, it is distributed under the terms of the      *)
+(*         GNU Lesser General Public License version 3                    *)
+(*              (see file LICENSE for more details)                       *)
 (*                                                                        *)
 (*       Copyright 2014: Jean-Guillaume Dumas, Dominique Duval            *)
-(*			 Burak Ekici, Damien Pous.                        *)
+(*             Burak Ekici, Damien Pous.                                  *)
 (**************************************************************************)
 
 Require Import Relations Morphisms.
@@ -13,134 +14,118 @@ Require Memory Terms Decorations Derived_Terms.
 Set Implicit Arguments.
 Require Import ZArith.
 Open Scope Z_scope.
+Require Import Bool.
 
 Module Make(Import M: Memory.T).
-  Module Export AxiomsExp := Derived_Terms.Make(M). 
+  Module Export AxiomsExp := Derived_Terms.Make(M).
 
  Reserved Notation "x == y" (at level 80).
  Reserved Notation "x ~~ y" (at level 80).
 
- Fixpoint chk_lt (a1 a2: Z) : Prop :=
-  match (a1 ?= a2)%Z with 
-    | Lt => True
-    | _  => False
-  end.
-
- Fixpoint chk_le (a1 a2: Z) : Prop :=
-  match (a1 ?= a2)%Z with 
-    | Gt => False
-    | _  => True
-  end.
-
- Fixpoint chk_gt (a1 a2: Z) : Prop :=
-  match (a1 ?= a2)%Z with 
-    | Gt => True
-    | _  => False
-  end.
-
- Fixpoint chk_ge (a1 a2: Z) : Prop :=
-  match (a1 ?= a2)%Z with 
-    | Lt => False
-    | _  => True
-  end.
-
- Fixpoint chk_eq (a1 a2: Z) : Prop :=
-  match (a1 ?= a2)%Z with 
-    | Eq => True
-    | _  => False
-  end.
-
- Fixpoint chk_neq (a1 a2: Z) : Prop :=
-  match (a1 ?= a2)%Z with 
-    | Eq => False
-    | _  => True
-  end.
-
- Inductive strong: forall X Y, relation (term X Y) := 
- | strong_refl: forall X Y (f: term X Y), f == f 
+ Inductive strong: forall X Y, relation (term X Y) :=
+ | strong_refl: forall X Y (f: term X Y), f == f
  | assoc: forall X Y Z T (f: term X Y) (g: term Y Z) (h: term Z T),
    f o (g o h) == (f o g) o h
- | id_src: forall X Y (f: term X Y), f o (@id Y) == f
- | id_tgt: forall X Y (f: term X Y), (@id X) o f == f
- | strong_subs: forall X Y Z (g1 g2: term X Y) (f: term Y Z), g1 == g2 -> g1 o f == g2 o f
- | strong_repl: forall X Y Z (g1 g2: term X Y) (f: term Z X), g1 == g2 -> f o g1 == f o g2
+ | id_src: forall X Y (f: term X Y), f o id == f
+ | id_tgt: forall X Y (f: term X Y), id o f == f
+
+ | sc: forall X Y Z, Proper (@strong X Y ==> @strong Y Z ==> @strong X Z) comp
+
  | one_weak_to_strong: forall X Y (f g: term X Y), is ro f -> is ro g -> f ~~ g -> f == g
 
- | strong_proj_pi2_rorw: forall X Y' Y (f1: term Y X) (f2: term Y' X),
-   is ro f1 -> (@pi2 Y Y') o pair f1 f2 == f2
+ | pure_pure: forall X Y Z (f: Y -> Z) (g: X -> Y),
+   tpure f o tpure g  == tpure (fun x => f (g x))
 
+ | pure_eq: forall X Y (f g: Y -> X),
+   (forall x, f x = g x) -> tpure f == tpure g
+
+ | strong_proj_pi2_rorw: forall X Y' Y (f1: term Y X) (f2: term Y' X),
+   is ro f1 -> pi2 o pair f1 f2 == f2
+
+ | observation: forall X (f g: term unit X),
+   (forall i: Loc, lookup i o f ~~ lookup i o g) -> f == g
+
+ | comp_final_unique: forall X Y (f g: term Y X),
+   forget o f == forget o g -> f ~~ g -> f == g
+	
  | strong_coproj_copi1_rwrw: forall X Y' Y (f1: term X Y) (f2: term X Y'),
    copair f1 f2 o (@copi1 Y Y') == f1 
 
  | strong_coproj_copi2_rwrw: forall X Y' Y (f1: term X Y) (f2: term X Y'),
    copair f1 f2 o (@copi2 Y Y') == f2 
 
- | observation: forall X (f g: term unit X),
-   (forall i: Loc, lookup i o f ~~ lookup i o g) -> f == g
-
- | comp_final_unique: forall X Y (f g: term Y X),
-   ((@forget Y) o f == (@forget Y) o g) -> f ~~ g -> f == g
-
- | counicity: forall  X Y Y'(f g: term X (Y/+/Y')),
+ | counicity: forall  X Y Y'(f g: term X (Y+Y')),
    (f o (@copi1 Y Y') ~~ g o (@copi1 Y Y')) -> (f o (@copi2 Y Y') ~~ g o (@copi2 Y Y')) -> f == g
 
- | IMP_IntAdd: forall p q: Z, 
-   plus o (pair (@constant Z p) (@constant Z q)) == (@constant Z (p+q))
- | IMP_IntMult: forall p q: Z, 
-   mult o (pair (@constant Z p) (@constant Z q)) == (@constant Z (p*q))
+ (* IMP Assumptions *)
+
+ | IMP_IntAdd: forall p q: Z,
+   tpure add o (pair (@constant Z p) (@constant Z q)) == (constant (add(p,q)))
+ | IMP_IntMult: forall p q: Z,
+   tpure mlt o (pair (@constant Z p) (@constant Z q)) == (constant (mlt(p,q)))
+
  | IMP_IntGtT: forall p q: Z,
-   (chk_gt p q) -> gt o (pair (@constant Z p) (@constant Z q)) == ttrue
+   Is_true(chkgt(p, q)) -> passbool  o tpure chkgt o (pair (@constant Z p) (@constant Z q)) == ttrue
  | IMP_IntGeT: forall p q: Z,
-   (chk_ge p q) -> ge o (pair (@constant Z p) (@constant Z q)) == ttrue
+    Is_true(chkge(p, q)) ->  passbool o tpure chkge o (pair (@constant Z p) (@constant Z q)) == ttrue
  | IMP_IntEqT: forall p q: Z,
-   (chk_eq p q) -> eq o (pair (@constant Z p) (@constant Z q)) == ttrue
+   Is_true(chkeq(p, q)) -> passbool  o tpure chkeq o (pair (@constant Z p) (@constant Z q)) == ttrue
+ | IMP_IntNeqT: forall p q: Z,
+   Is_true(chkneq(p, q)) -> passbool  o tpure chkneq o (pair (@constant Z p) (@constant Z q)) == ttrue
  | IMP_IntLtT: forall p q: Z,
-   (chk_lt p q) -> lt o (pair (@constant Z p) (@constant Z q)) == ttrue
+   Is_true(chklt(p, q)) -> passbool o tpure chklt o (pair (@constant Z p) (@constant Z q)) == ttrue
  | IMP_IntLeT: forall p q: Z,
-   (chk_le p q) -> le o (pair (@constant Z p) (@constant Z q)) == ttrue
+   Is_true(chkle(p, q)) -> passbool o tpure chkle o (pair (@constant Z p) (@constant Z q)) == ttrue
 
  | IMP_IntGtF: forall p q: Z,
-   (chk_le p q) -> gt o (pair (@constant Z p) (@constant Z q)) == ffalse
+   Is_true(chkle(p, q)) -> passbool  o tpure chkgt o (pair (@constant Z p) (@constant Z q)) == ffalse
+
  | IMP_IntGeF: forall p q: Z,
-   (chk_lt p q) -> ge o (pair (@constant Z p) (@constant Z q)) == ffalse
+   Is_true(chklt(p, q)) -> passbool  o tpure chkge o (pair (@constant Z p) (@constant Z q)) == ffalse
  | IMP_IntEqF: forall p q: Z,
-   (chk_neq p q) -> eq o (pair (@constant Z p) (@constant Z q)) == ffalse
+   Is_true(chkneq(p, q)) -> passbool  o tpure chkeq o (pair (@constant Z p) (@constant Z q)) == ffalse
+ | IMP_IntNeqF: forall p q: Z,
+   Is_true(chkeq(p, q)) -> passbool  o tpure chkneq o (pair (@constant Z p) (@constant Z q)) == ffalse
  | IMP_IntLtF: forall p q: Z,
-   (chk_ge p q) -> lt o (pair (@constant Z p) (@constant Z q)) == ffalse
+   Is_true(chkge(p, q)) -> passbool o tpure chklt o (pair (@constant Z p) (@constant Z q)) == ffalse
+
  | IMP_IntLeF: forall p q: Z,
-   (chk_gt p q) -> le o (pair (@constant Z p) (@constant Z q)) == ffalse
+   Is_true(chkgt(p, q)) -> passbool o tpure chkle o (pair (@constant Z p) (@constant Z q)) == ffalse
 
- | IMP_IntAndT: forall p q: term boolT unit,
-   pi1 o (pair p q) == ttrue -> pi2 o (pair p q) == ttrue -> andB o (pair p q) == ttrue
- | IMP_IntAndF: forall p q: term boolT unit,
-   pi1 o (pair p q) == ffalse \/ pi2 o (pair p q) == ffalse -> andB o (pair p q) == ffalse
+ | IMP_IntAndT: forall p q: bool,
+   p = true -> q = true -> passbool  o tpure ve o (pair (@constant bool p) (@constant bool q)) == ttrue
+ | IMP_IntAndF: forall p q: bool,
+   p = false \/ q = false -> passbool  o tpure ve o (pair (@constant bool p) (@constant bool q)) == ffalse
 
- | IMP_IntOrF: forall p q: term boolT unit,
-   pi1 o (pair p q) == ffalse -> pi2 o (pair p q) == ffalse -> orB o (pair p q) == ffalse
- | IMP_IntOrT: forall p q: term boolT unit,
-   pi1 o (pair p q) == ttrue \/ pi2 o (pair p q) == ttrue -> orB o (pair p q) == ttrue
+ | IMP_IntOrF: forall p q: bool,
+   p = false -> q = false -> passbool  o tpure yada o (pair (@constant bool p) (@constant bool q)) == ffalse
+ | IMP_IntOrT: forall p q: bool,
+   p = true \/ q = true -> passbool  o tpure yada o (pair (@constant bool p) (@constant bool q)) == ttrue 
 
- | IMP_Loop: forall (b: term boolT unit) (f w: term unit unit),
-   w == (copair (w o f) id) o b
+ | IMP_Loop: forall (b: term (unit+unit) unit) (f : term unit unit),
+   loopdec b f == (copair ((loopdec b f) o f) id) o b 
+
+ (* \IMP Assumptions *)
 
  | strong_sym: forall X Y, Symmetric (@strong X Y)
  | strong_trans: forall X Y, Transitive (@strong X Y)
- with weak: forall X Y, relation (term X Y) := 
- | weak_subs: forall X Y Z (g1 g2: term X Y) (f: term Y Z), g1 ~~ g2 -> g1 o f ~~ g2 o f
- | zero_weak_repl: forall X Y Z (g: term X Y) (f1 f2: term Y Z),
-   is pure g -> f1 ~~ f2 -> g o f1 ~~ g o f2
+ with weak: forall X Y, relation (term X Y) :=
+ | wsc: forall A B C,
+               Proper (@weak C B ==> @strong  B A ==> @weak C A) comp
+ | wrc: forall A B C (g: term C B), (PURE g) ->
+               Proper (@weak B A ==> @weak C A) (comp g)
 
- | weak_final_unique: forall X (f g: term unit X), f ~~ g	
+ | weak_final_unique: forall X (f g: term unit X), f ~~ g    
 
- | axiom_1: forall i, lookup i o update i ~~ (@id Z)
- | axiom_2: forall i j, i<>j -> lookup j o update i ~~ lookup j o (@forget Z)
+ | axiom_1: forall i, lookup i o update i ~~ id
+ | axiom_2: forall i j, i<>j -> lookup j o update i ~~ lookup j o forget
  | strong_to_weak: forall  X Y (f g: term X Y), f == g -> f ~~ g
 
- | weak_proj_pi1_rorw: forall X Y' Y (f1: term Y X) (f2: term Y' X), 
-   is ro f1 -> (@pi1 Y Y') o pair f1 f2 ~~ f1
+ | weak_proj_pi1_rorw: forall X Y' Y (f1: term Y X) (f2: term Y' X),
+   is ro f1 -> pi1 o pair f1 f2 ~~ f1
 
- | unicity: forall  X Y Y'(f g: term (Y/*/Y') X),
-   ((@pi1 Y Y') o f ~~ (@pi1 Y Y') o g) -> ((@pi2 Y Y') o f ~~ (@pi2 Y Y') o g) -> f ~~ g
+ | unicity: forall  X Y Y'(f g: term (Y*Y') X),
+   pi1 o f ~~ pi1 o g -> pi2 o f ~~ pi2 o g -> f ~~ g
 
  | weak_sym: forall X Y, Symmetric (@weak X Y)
  | weak_trans: forall X Y, Transitive (@weak X Y)
@@ -165,8 +150,72 @@ Module Make(Import M: Memory.T).
  Qed.
 
  Instance strong_is_weak_equivalence: forall X Y, subrelation (@strong X Y) (@weak X Y).
- Proof.
-     constructor. assumption.
- Qed.
+ Proof. constructor. assumption. Qed.
 
+ Existing Instance wsc.
+ Existing Instance wrc.
+ Existing Instance sc.
+
+ Ltac catpr :=
+   match goal with
+      | H: _ |-  pi1 o pair ?f1 ?f2 ~~ ?f1
+        => apply weak_proj_pi1_rorw; decorate
+      | H: _ |-  pi2 o pair ?f1 ?f2 == ?f2
+        => apply strong_proj_pi2_rorw; decorate
+      | H: _ |-  pi1 o prod ?f ?g ~~ ?f o pi1
+        => apply weak_proj_pi1_rorw; decorate
+      | H: _ |-  pi2 o prod ?f ?g == ?g o pi2
+        => apply strong_proj_pi2_rorw; decorate
+   end. 
+ 
 End Make.
+
+
+(*
+
+	(* IMP *)
+
+ | IMP_IntGtT: forall p q: Z,
+   (p > q) -> gt o (pair (@constant Z p) (@constant Z q)) == ttrue
+ | IMP_IntGeT: forall p q: Z,
+   (p > q) \/ (p = q) -> ge o (pair (@constant Z p) (@constant Z q)) == ttrue
+ | IMP_IntEqT: forall p q: Z,
+   (p = q) -> eq o (pair (@constant Z p) (@constant Z q)) == ttrue
+ | IMP_IntNeqT: forall p q: Z,
+   (p <> q) -> neq o (pair (@constant Z p) (@constant Z q)) == ttrue
+ | IMP_IntLtT: forall p q: Z,
+   (p < q) -> lt o (pair (@constant Z p) (@constant Z q)) == ttrue
+ | IMP_IntLeT: forall p q: Z,
+   (p < q) \/ (p = q) -> le o (pair (@constant Z p) (@constant Z q)) == ttrue
+
+ | IMP_IntGtF: forall p q: Z,
+   (p < q) \/ (p = q) -> gt o (pair (@constant Z p) (@constant Z q)) == ffalse
+
+ | IMP_IntGeF: forall p q: Z,
+   (p < q) -> ge o (pair (@constant Z p) (@constant Z q)) == ffalse
+ | IMP_IntEqF: forall p q: Z,
+   (p <> q) -> eq o (pair (@constant Z p) (@constant Z q)) == ffalse
+ | IMP_IntNeqF: forall p q: Z,
+   (p = q) -> neq o (pair (@constant Z p) (@constant Z q)) == ffalse
+ | IMP_IntLtF: forall p q: Z,
+   (p > q) \/ (p = q) -> lt o (pair (@constant Z p) (@constant Z q)) == ffalse
+
+ | IMP_IntLeF: forall p q: Z,
+   (p > q) -> le o (pair (@constant Z p) (@constant Z q)) == ffalse
+ | IMP_IntAndT: forall p q: term boolT unit,
+   pi1 o (pair p q) == ttrue -> pi2 o (pair p q) == ttrue -> andB o (pair p q) == ttrue
+ | IMP_IntAndF: forall p q: term boolT unit,
+   pi1 o (pair p q) == ffalse \/ pi2 o (pair p q) == ffalse -> andB o (pair p q) == ffalse
+
+ | IMP_IntOrF: forall p q: term boolT unit,
+   pi1 o (pair p q) == ffalse -> pi2 o (pair p q) == ffalse -> orB o (pair p q) == ffalse
+ | IMP_IntOrT: forall p q: term boolT unit,
+   pi1 o (pair p q) == ttrue \/ pi2 o (pair p q) == ttrue -> orB o (pair p q) == ttrue
+
+ | IMP_Loop: forall (b: term boolT unit) (f : term unit unit),
+   loopdec b f == (copair ((loopdec b f) o f) id) o b
+   
+	(* End IMP *)
+
+*)
+
