Decorations.v
@@ -1,7 +1,7 @@
 (**************************************************************************)
-(*  This is part of IMP-STATES, it is distributed under the terms of the  *)
-(*              GNU Lesser General Public License version 3               *)
-(*                  (see file LICENSE for more details)                   *)
+(*  This is part of STATES, it is distributed under the terms of the      *)
+(*         GNU Lesser General Public License version 3                    *)
+(*              (see file LICENSE for more details)                       *)
 (*                                                                        *)
 (*       Copyright 2014: Jean-Guillaume Dumas, Dominique Duval            *)
 (*			 Burak Ekici, Damien Pous.                        *)
@@ -13,37 +13,43 @@ Require Memory Terms.
 Set Implicit Arguments.
 Require Import ZArith.
 Open Scope Z_scope.
+Require Import Bool.
 
 Module Make(Import M: Memory.T).
   Module Export DecorationsExp := Terms.Make(M). 
 
- Inductive kind := pure | ro | rw. 
+ Inductive kind := pure | ro | rw.
 
-Inductive is: kind -> forall X Y, term X Y -> Prop :=
- | is_id: forall X, is pure (@id X)
- | is_comp: forall k X Y Z (f: term X Y) (g: term Y Z), is k f -> is k g -> is k (f o g)
- | is_forget: forall X, is pure (@forget X)
- | is_pair: forall k X Y Z (f: term X Z) (g: term Y Z), is k f -> is k g -> is k (pair f g)
- | is_copair: forall k X Y Z (f: term Z X) (g: term Z Y), is k f -> is k g -> is k (copair f g) 
- | is_pi1: forall X Y, is pure (@pi1 X Y)
- | is_pi2: forall X Y, is pure (@pi2 X Y)
- | is_copi1: forall X Y, is pure (@copi1 X Y) 
- | is_copi2: forall X Y, is pure (@copi2 X Y)
- | is_plus: forall X, is pure (@plus X)
- | is_mult: forall X, is pure (@mult X)
- | is_gt: is pure gt
- | is_ge: is pure ge
- | is_lt: is pure lt
- | is_le: is pure le
- | is_eq: is pure eq
- | is_andB: is pure andB
- | is_orB: is pure orB
- | is_constant: forall X: Set, forall c: X, is pure (@constant X c)
- | is_lookup: forall i, is ro (lookup i)   
- | is_update: forall i, is rw (update i)
- | is_pure_ro: forall X Y (f: term X Y), is pure f -> is ro f
- | is_ro_rw: forall X Y  (f: term X Y), is ro f -> is rw f.
+ Inductive is: kind -> forall X Y, term X Y -> Prop :=
+  | is_tpure: forall X Y (f: X -> Y), is pure (@tpure X Y f)
+  | is_comp: forall k X Y Z (f: term X Y) (g: term Y Z), is k f -> is k g -> is k (f o g)
+  | is_pair: forall k X Y Z (f: term X Z) (g: term Y Z), is k f -> is k g -> is k (pair f g)
+  | is_copair: forall k X Y Z (f: term Z X) (g: term Z Y), is k f -> is k g -> is k (copair f g) 
+  | is_lookup: forall i, is ro (lookup i)   
+  | is_update: forall i, is rw (update i)
+  | is_pure_ro: forall X Y (f: term X Y), is pure f -> is ro f
+  | is_ro_rw: forall X Y  (f: term X Y), is ro f -> is rw f.
 
  Hint Constructors is.
 
+ Ltac decorate :=  solve[
+                          repeat (apply is_comp || apply is_pair)
+                            ||
+		                 (apply is_tpure || apply is_lookup || apply is_update || assumption)
+			    || 
+                                 (apply is_pure_ro)
+			    || 
+		                 (apply is_ro_rw)
+                        ].
+
+ Class PURE {A B: Type} (f: term A B) := isp : is pure f.
+ Hint Extern 0 (PURE _) => decorate : typeclass_instances.
+
+ Class RO {A B: Type} (f: term A B) := isro : is ro f.
+ Hint Extern 0 (RO _) => decorate : typeclass_instances.
+
+ Class RW {A B: Type} (f: term A B) := isrw : is rw f.
+ Hint Extern 0 (RW _) => decorate : typeclass_instances.
+
 End Make.
+
