Derived_Terms.v
@@ -1,7 +1,7 @@
 (**************************************************************************)
-(*  This is part of IMP-STATES, it is distributed under the terms of the  *)
-(*              GNU Lesser General Public License version 3               *)
-(*                  (see file LICENSE for more details)                   *)
+(*  This is part of STATES, it is distributed under the terms of the      *)
+(*         GNU Lesser General Public License version 3                    *)
+(*              (see file LICENSE for more details)                       *)
 (*                                                                        *)
 (*       Copyright 2014: Jean-Guillaume Dumas, Dominique Duval            *)
 (*			 Burak Ekici, Damien Pous.                        *)
@@ -11,19 +11,213 @@ Require Import Relations Morphisms.
 Require Import Program.
 Require Memory Terms Decorations.
 Set Implicit Arguments.
+Require Import ZArith.
+Open Scope Z_scope.
+Require Import Bool.
 
 Module Make(Import M: Memory.T).
-  Module Export Derived_TermsExp := Decorations.Make(M). 
+  Module Export Derived_TermsExp := Decorations.Make(M).
 
- (*For states*)
+ Definition id  {X: Type}     : term X X       := tpure id.
+ Definition pi1 {X Y: Type}   : term X (X*Y)   := tpure fst. 
+ Definition pi2 {X Y: Type}   : term Y (X*Y)   := tpure snd.
+ Definition forget {X}        : term unit X    := tpure (fun _ => tt).
+(* Definition constant (v: Z)   : term Z unit    := tpure (fun _ => v).
+   Definition constant {X Y: Type} (v: Y): term Y X := tpure (fun _ => v). *)
 
- Definition ttrue:  term boolT unit := (@copi1 unit unit).
- Definition ffalse: term boolT unit := (@copi2 unit unit). 
+ Definition loopdec (b: term (unit+unit) unit) (f: term unit unit) : term unit unit  
+    := tpure(fun tt => tt).
+
+ Definition copi1 {X Y}       : term (X+Y) X  := tpure inl.
+ Definition copi2 {X Y}       : term (X+Y) Y  := tpure inr. 
+ Definition empty {X} (x: X)  : term X empty_set:= tpure (fun _ => x).
+ Definition constant {X: Type} (v: X): term X unit := tpure (fun _ => v). 
+
+ Definition add (p: Z * Z) := match p with
+                                | (x, y) => x + y
+                              end.
+
+ Definition mlt (p: Z * Z) := match p with
+                                | (x, y) => x * y
+                              end.
+
+
+ Definition chkgt (p: Z * Z) : bool := match p with
+                                              | (a1, a2) => match (a1 ?= a2)%Z with 
+                                                              | Gt => true
+                                                              | _  => false
+                                                            end
+                                            end.
+
+
+
+ Definition chkge (p: Z * Z) : bool := match p with
+                                              | (a1, a2) => match (a1 ?= a2)%Z with 
+                                                              | Lt => false
+                                                              | _  => true
+                                                           end
+                                            end.
+
+ Definition chklt (p: Z * Z) : bool := match p with
+                                              | (a1, a2) => match (a1 ?= a2)%Z with 
+                                                              | Lt => true
+                                                              | _  => false
+                                                            end
+                                            end.
+
+ Definition chkle (p: Z * Z) : bool := match p with
+                                              | (a1, a2) => match (a1 ?= a2)%Z with 
+                                                              | Gt => false
+                                                              | _  => true
+                                                            end
+                                            end.
+
+ Definition chkeq (p: Z * Z) : bool := match p with
+                                              | (a1, a2) => match (a1 ?= a2)%Z with 
+                                                              | Eq => true
+                                                              | _  => false
+                                                            end
+                                            end.
+
+ Definition chkneq (p: Z * Z) : bool := match p with
+                                               | (a1, a2) => match (a1 ?= a2)%Z with 
+                                                               | Eq => false
+                                                               | _  => true
+                                                             end
+                                             end.
+
+ Definition ve (p: bool * bool): bool := match p with
+                                                | (x, y) => match (x && y) with 
+                                                               | false => false
+                                                               | true  => true
+                                                             end
+                                              end.
+
+ Definition yada (p: bool * bool): bool := match p with
+                                                  | (x, y) => match (x || y) with 
+                                                                | false => false
+                                                                | true  => true
+                                                              end
+                                                end.
+
+ Definition bool_to_two (b: bool): unit + unit :=
+    match b with
+       | false => inr tt
+       | true  => inl tt
+    end.
+
+ Definition bool_to_prop (b: bool): Prop :=
+     match b with
+       | false => False
+       | true  => True
+    end.
+
+ Check tt.
+
+ Definition passbool: term (unit + unit) bool := tpure bool_to_two.
+ 
+ Definition prod_forget {X Y}: term unit (X*Y) := forget.
+ Definition iso {X}: term (X*unit) X := pair id forget. 
+ Definition inv_pi1 {X}: term (X*unit) X := pair id forget. 
+ Definition permut {X Y}: term (X*Y) (Y*X) := pair pi2 pi1.
+ 
+ Definition perm_pair {X Y Z} (f: term Y X) (g: term Z X): term (Y*Z) X
+ := permut o pair g f.
+ Definition prod {X Y X' Y'} (f: term X X') (g: term Y Y'): term (X*Y) (X'*Y')
+ := pair (f o pi1) (g o pi2).
+ Definition perm_prod {X Y X' Y'} (f: term X X') (g: term Y Y') := permut o pair (g o pi2) (f o pi1).
+ (*Definition perm_prod {X Y X' Y'} (f: term X X') (g: term Y Y'): term (X*Y) (X'*Y')
+ := perm_pair (f o pi1) (g o pi2).*)
+
+ Definition ttrue  : term (unit+unit) unit := copi1.
+ Definition ffalse : term (unit+unit) unit := copi2.
+
+ Lemma is_loopdec: forall k (b: term (unit+unit) unit) (f: term unit unit),
+ is k b -> is k f -> is pure (loopdec b f).
+ Proof. intros. decorate. Qed.
+
+ Lemma is_prod_forget X Y: is pure (@prod_forget X Y).
+ Proof. decorate. Qed.
+
+ Lemma is_inv_pi1 X: is pure (@inv_pi1 X).
+ Proof. decorate. Qed.
+ 
+ Lemma is_permut X Y: is pure (@permut X Y).
+ Proof. decorate. Qed.
+
+ Lemma is_perm_pair: forall k X Y Z (f: term Y X) (g: term Z X),
+ is k f -> is k g -> is k (perm_pair f g).
+ Proof. intros. induction k; decorate. Qed.
+
+ Lemma is_prod: forall k X' X Y' Y (f: term X X') (g: term Y Y'), 
+ is k f -> is k g -> is k (prod f g).
+ Proof. intros. induction k; decorate. Qed. 
+
+ Lemma is_perm_prod: forall k X' X Y' Y (f: term X X') (g: term Y Y'), 
+ is k f -> is k g -> is k (perm_prod f g).
+ Proof. intros. induction k; decorate. Qed.
 
  Lemma is_ttrue: is pure (@copi1 unit unit).
- Proof. auto. Qed.
+ Proof. decorate. Qed.
 
  Lemma is_ffalse: is pure (@copi2 unit unit).
- Proof. auto. Qed.
- 
+ Proof. decorate. Qed.
+
+ Lemma is_id X: is pure (@id X).
+ Proof. decorate. Qed.
+
+ Lemma is_pi1 X Y: is pure (@pi1 X Y).
+ Proof. decorate. Qed.
+
+ Lemma is_pi2 X Y: is pure (@pi2 X Y).
+ Proof. decorate. Qed.
+
+ Lemma is_forget X: is pure (@forget X).
+ Proof. apply is_tpure. Qed.
+
+ Lemma is_constant (v: Z): is pure (constant v).
+ Proof. apply is_tpure. Qed.
+
+ Lemma is_copi1 X Y: is pure (@copi1 X Y).
+ Proof. decorate. Qed.
+
+ Lemma is_copi2 X Y: is pure (@copi2 X Y).
+ Proof. decorate. Qed.
+
+ Lemma is_empty {X: Type} (x: X): is pure (@empty X x).
+ Proof. decorate. Qed.
+
+(* Lemma is_plus: is pure (plus).
+ Proof. decorate. Qed.
+
+ Lemma is_mult: is pure (mult).
+ Proof. decorate. Qed.
+
+ Lemma is_gt: is pure (gt).
+ Proof. decorate. Qed.
+
+ Lemma is_ge: is pure (ge).
+ Proof. decorate. Qed.
+
+ Lemma is_lt: is pure (lt).
+ Proof. decorate. Qed.
+
+ Lemma is_le: is pure (le).
+ Proof. decorate. Qed.
+
+ Lemma is_eq: is pure (eq).
+ Proof. decorate. Qed.
+
+ Lemma is_neq: is pure (neq).
+ Proof. decorate. Qed.
+
+ Lemma is_and: is pure (and).
+ Proof. decorate. Qed.
+
+ Lemma is_or: is pure (or).
+ Proof. decorate. Qed. *)
+
+ Lemma is_passbool: is pure (passbool).
+ Proof. decorate. Qed.
+
 End Make.
