Terms.v
@@ -1,7 +1,7 @@
 (**************************************************************************)
-(*  This is part of IMP-STATES, it is distributed under the terms of the  *)
-(*              GNU Lesser General Public License version 3               *)
-(*                  (see file LICENSE for more details)                   *)
+(*  This is part of STATES, it is distributed under the terms of the      *)
+(*         GNU Lesser General Public License version 3                    *)
+(*              (see file LICENSE for more details)                       *)
 (*                                                                        *)
 (*       Copyright 2014: Jean-Guillaume Dumas, Dominique Duval            *)
 (*			 Burak Ekici, Damien Pous.                        *)
@@ -13,48 +13,21 @@ Require Memory.
 Set Implicit Arguments.
 Require Import ZArith.
 Open Scope Z_scope.
+Require Import Bool.
 
 Module Make(Import M: Memory.T).
 
- Variable coproductT: Type -> Type -> Type.
- Notation "y '/+/' z" := (coproductT y z) (at level 70).
-
- Variable productT: Type -> Type -> Type.
- Notation "y '/*/' z" := (productT y z) (at level 70).
-
- Definition boolT: Type := (unit/+/unit).
+ Inductive empty_set : Set :=.
 
  Inductive term: Type -> Type -> Type :=
-  | id: forall {X}, term X X
-  | comp: forall {X Y Z}, term X Y -> term Y Z -> term X Z
-  | downcast: forall {X Y} (f: term X Y), term X Y 
-  | forget: forall {X}, term unit X
-  | empty: forall {X}, term X empty_set
-  | pair: forall {X Y Z}, term X Z -> term Y Z -> term (X/*/Y) Z
-  | copair: forall {X Y Z}, term Z X -> term Z Y -> term Z (X/+/Y) 	
-  | pi1: forall {X Y}, term X (X/*/Y)
-  | pi2: forall {X Y}, term Y (X/*/Y)
-  | copi1: forall {X Y}, term (X/+/Y) X
-  | copi2: forall {X Y}, term (X/+/Y) Y
-  | loopdec: term unit unit
-  | plus: forall {X}, term X (X/*/X) 
-  | mult: forall {X}, term X (X/*/X)	
-  | gt: term boolT (Z/*/Z)
-  | lt: term boolT (Z/*/Z)
-  | ge: term boolT (Z/*/Z)
-  | le: term boolT (Z/*/Z)
-  | eq: term boolT (Z/*/Z)
-  | andB: term boolT (boolT/*/boolT)
-  | orB: term boolT (boolT/*/boolT)
-  | constant: forall (X: Set), X -> term X unit 
-  | lookup: Loc -> term Z unit
-  | update: Loc -> term unit Z
-  | tag: EName -> term empty_set unit	
-  | untag: EName -> term unit empty_set.
+  | comp:   forall {X Y Z: Type}, term X Y -> term Y Z -> term X Z
+  | pair: forall {X Y Z: Type}, term X Z -> term Y Z -> term (X*Y) Z
+  | copair: forall {X Y Z}, term Z X -> term Z Y -> term Z (X+Y) 
+  | tpure:  forall {X Y: Type}, (X -> Y) -> term Y X
+  | lookup: forall i:Loc, term Z unit    
+  | update: forall i:Loc, term unit Z.
 
  Infix "o" := comp (at level 70).
-
-
 
 End Make.
 
