Derived_Pairs.v
@@ -1,0 +1,234 @@
+(**************************************************************************)
+(*  This is part of STATES, it is distributed under the terms of the      *)
+(*         GNU Lesser General Public License version 3                    *)
+(*              (see file LICENSE for more details)                       *)
+(*                                                                        *)
+(*       Copyright 2014: Jean-Guillaume Dumas, Dominique Duval            *)
+(*			 Burak Ekici, Damien Pous.                        *)
+(**************************************************************************)
+
+Require Import Relations Morphisms.
+Require Import Program.
+Require Memory Terms Decorations Derived_Terms Axioms.
+Set Implicit Arguments.
+Require Import ZArith.
+Open Scope Z_scope.
+Require Import Bool.
+
+Module Make(Import M: Memory.T).
+  Module Export Derived_PairsExp := Axioms.Make(M). 
+
+(* --- Derived Pair Existencies --- *)
+
+ (* --- A pair of modifiers: Existence --- *) 
+
+ Lemma dec_pair_exists_rwrw: forall X Y Y' (f1: term Y X) (f2: term Y' X),
+ RW f1 -> RW f2 -> RW (pair f1 f2).
+ Proof. intros. decorate. Qed.
+
+ Lemma dec_perm_pair_exists_rwrw: forall X Y Y' (f1: term Y X) (f2: term Y' X),
+ RW f2 -> RW f1 -> RW (perm_pair f1 f2).
+ Proof. intros. decorate. Qed.
+
+ (* --- An accessor and a modifier: Existence --- *)
+
+ Lemma dec_pair_exists_rorw: forall X Y Y' (f1: term Y X) (f2: term Y' X),
+ RO f1 -> RW f2 -> RW (pair f1 f2).
+ Proof. intros. decorate. Qed.
+
+ Lemma dec_perm_pair_exists_rwro: forall X Y Y' (f1: term Y X) (f2: term Y' X),
+ RO f2 -> RW f1 -> RW (perm_pair f1 f2).
+ Proof. intros. decorate. Qed.
+
+ (* --- A pure function and a modifier: Existence*)
+
+ Lemma dec_pair_exists_purerw: forall X Y Y' (f1: term Y X) (f2: term Y' X),
+ PURE f1 -> RW f2 -> RW (pair f1 f2).
+ Proof. intros. decorate. Qed.
+
+ Lemma dec_perm_pair_exists_rwpure: forall X Y Y' (f1: term Y X) (f2: term Y' X),
+ PURE f2 -> RW f1 -> RW (perm_pair f1 f2).
+ Proof. intros. decorate. Qed.
+
+ (* --- A pair of accessors: Existence --- *) 
+
+ Lemma dec_pair_exists_roro: forall X Y Y' (f1: term Y X) (f2: term Y' X),
+ RO f1 -> RO f2 -> RO (pair f1 f2).
+ Proof. intros. decorate. Qed.
+
+ Lemma dec_perm_pair_exists_roro: forall X Y Y' (f1: term Y X) (f2: term Y' X),
+ RO f2 -> RO f1 -> RO (perm_pair f1 f2).
+ Proof. intros. decorate. Qed.
+
+ (* --- A pure function and an accessor: Existence --- *) 
+
+ Lemma dec_pair_exists_purero: forall X Y Y' (f1: term Y X) (f2: term Y' X),
+ PURE f1 -> RO f2 -> RO (pair f1 f2).
+ Proof. intros. decorate. Qed.
+
+ Lemma dec_perm_pair_exists_ropure: forall X Y Y' (f1: term Y X) (f2: term Y' X),
+ PURE f2 -> RO f1 -> RO (perm_pair f1 f2).
+ Proof. intros. decorate. Qed.
+
+ (* --- A pair of pure functions: Existence --- *) 
+
+ Lemma dec_pair_exists_purepure: forall X Y Y' (f1: term Y X) (f2: term Y' X),
+ PURE f1 -> PURE f2 -> PURE (pair f1 f2).
+ Proof. intros. decorate. Qed.
+
+ Lemma dec_perm_pair_exists_purepure: forall X Y Y' (f1: term Y X) (f2: term Y' X),
+ PURE f2 -> PURE f1 -> PURE (perm_pair f1 f2).
+ Proof. intros. decorate. Qed.
+
+(* -------------------- End of Derived Pair Existencies -------------------- *)
+
+(* --- Derived Pair Projections: --- *)
+
+(* --- A pair of modifiers: Projections --- *) 
+
+ (* ...Nothing to be proven... *)
+
+
+ (* --- A pair of pure functions: Projections --- *) 
+
+ Lemma strong_proj_pi1_purepure: forall X Y' Y (f1: term Y X) (f2: term Y' X),
+   PURE f1 -> PURE f2 -> pi1 o pair f1 f2 == f1.
+ Proof.
+     intros. apply one_weak_to_strong; (decorate || idtac).
+     apply weak_proj_pi1_rorw; decorate.
+ Qed.
+
+ Lemma strong_proj_pi2_purepure: forall X Y' Y (f1: term Y X) (f2: term Y' X),
+   PURE f1 ->  PURE f2 -> pi2 o pair f1 f2 == f2.
+ Proof. intros. apply strong_proj_pi2_rorw; decorate. Qed.
+
+ Lemma strong_perm_proj_pi1_purepure: forall X Y' Y (f1: term Y X) (f2: term Y' X),
+   PURE f2 -> PURE f1 -> pi1 o perm_pair f1 f2 == f1.
+ Proof.
+     intros. unfold perm_pair. unfold permut.
+     apply one_weak_to_strong; try decorate. rewrite assoc.
+     remember wsc. rewrite weak_proj_pi1_rorw; (solve[decorate] || idtac).
+     apply strong_to_weak. apply strong_proj_pi2_rorw; decorate.
+ Qed.
+
+ Lemma strong_perm_proj_pi2_purepure: forall X Y' Y (f1: term Y X) (f2: term Y' X),
+  PURE f2 ->  PURE f1 -> pi2 o perm_pair f1 f2 == f2.
+ Proof.
+     intros. unfold perm_pair. unfold permut. rewrite assoc.
+     remember sc. rewrite strong_proj_pi2_rorw; (solve[decorate] || idtac).
+     apply one_weak_to_strong; (solve[decorate] || idtac).
+     apply weak_proj_pi1_rorw; decorate.
+ Qed.
+
+ (* --- A pure function and an accessor: Projections --- *) 
+
+ Lemma strong_proj_pi1_purero: forall X Y' Y (f1: term Y X) (f2: term Y' X),
+   PURE f1 -> RO f2 -> pi1 o pair f1 f2 == f1.
+ Proof.
+     intros. apply one_weak_to_strong; (solve[decorate] || idtac).
+     apply weak_proj_pi1_rorw; decorate.
+ Qed.
+
+ Lemma strong_proj_pi2_purero: forall X Y' Y (f1: term Y X) (f2: term Y' X),
+   PURE f1 ->  RO f2 -> pi2 o pair f1 f2 == f2.
+ Proof. intros. apply strong_proj_pi2_rorw; decorate. Qed.
+
+ Lemma strong_perm_proj_pi1_ropure: forall X Y' Y (f1: term Y X) (f2: term Y' X),
+   PURE f2 -> RO f1 -> pi1 o perm_pair f1 f2 == f1.
+ Proof.
+     intros. (*unfold perm_pair. unfold permut. rewrite assoc.    
+     remember sc. apply one_weak_to_strong; (solve[decorate] || idtac).
+     rewrite weak_proj_pi1_rorw; (solve[decorate] || idtac).
+     apply strong_to_weak. apply strong_proj_pi2_rorw; decorate. *)
+     unfold perm_pair. unfold permut. rewrite assoc.    
+     remember sc. rewrite strong_proj_pi1_purepure; (solve[decorate] || idtac).
+     apply strong_proj_pi2_rorw; decorate. 
+ Qed.
+
+ Lemma strong_perm_proj_pi2_ropure: forall X Y' Y (f1: term Y X) (f2: term Y' X),
+  PURE f2 -> RO f1 -> pi2 o perm_pair f1 f2 == f2.
+ Proof.
+     intros. unfold perm_pair. unfold permut. rewrite assoc.
+     remember sc. rewrite strong_proj_pi2_purepure; try decorate.
+     apply one_weak_to_strong; try decorate.
+     apply weak_proj_pi1_rorw; decorate.
+ Qed.
+
+ (* --- A pair of accessors: Projections --- *) 
+
+ Lemma strong_proj_pi1_roro: forall X Y' Y (f1: term Y X) (f2: term Y' X),
+   RO f1 ->  RO f2 -> pi1 o pair f1 f2 == f1.
+ Proof.
+     intros. apply one_weak_to_strong; (solve[decorate] || idtac).
+     apply weak_proj_pi1_rorw; decorate.
+ Qed.
+
+ Lemma strong_proj_pi2_roro: forall X Y' Y (f1: term Y X) (f2: term Y' X),
+   RO f1 ->  RO f2 -> pi2 o pair f1 f2 == f2.
+ Proof. intros. apply strong_proj_pi2_rorw; decorate. Qed.
+
+ Lemma strong_perm_proj_pi1_roro: forall X Y' Y (f1: term Y X) (f2: term Y' X),
+   RO f2 ->  RO f1 -> pi1 o perm_pair f1 f2 == f1.
+ Proof.
+     intros. unfold perm_pair. unfold permut. rewrite assoc.
+     remember sc. rewrite strong_proj_pi1_purepure; (solve[decorate] || idtac). 
+     apply strong_proj_pi2_rorw; decorate. 
+ Qed.
+
+ Lemma strong_perm_proj_pi2_roro: forall X Y' Y (f1: term Y X) (f2: term Y' X),
+  RO f2 ->  RO f1 -> pi2 o perm_pair f1 f2 == f2.
+ Proof.
+     intros. unfold perm_pair. unfold permut. rewrite assoc.
+     remember sc. rewrite strong_proj_pi2_purepure; (solve[decorate] || idtac).
+     apply one_weak_to_strong; (solve[decorate] || idtac).
+     apply weak_proj_pi1_rorw; decorate. 
+ Qed.
+
+(* --- An accessor and a modifier: Projections --- *) 
+
+ Lemma strong_perm_proj_pi1_rwro: forall X Y' Y (f1: term Y X) (f2: term Y' X),
+   RO f2 -> pi1 o perm_pair f1 f2 == f1.
+ Proof.
+     intros. unfold perm_pair. unfold permut. rewrite assoc.
+     remember sc. rewrite strong_proj_pi1_purepure; (solve[decorate] || idtac). 
+     apply strong_proj_pi2_rorw; decorate. 
+ Qed.
+
+ Lemma weak_perm_proj_pi2_rwro: forall X Y' Y (f1: term Y X) (f2: term Y' X),
+   RO f2 -> pi2 o perm_pair f1 f2 ~~ f2.
+ Proof.
+     intros. unfold perm_pair. unfold permut. rewrite assoc.
+     remember wsc. rewrite strong_proj_pi2_purepure; (solve[decorate] || idtac). 
+     apply weak_proj_pi1_rorw; decorate.
+ Qed.
+
+ (* --- A pure function and a modifier: Projections --- *) 
+
+ Lemma weak_proj_pi1_purerw: forall X Y' Y (f1: term Y X) (f2: term Y' X),
+   PURE f1 -> pi1 o pair f1 f2 ~~ f1.
+ Proof. intros. apply weak_proj_pi1_rorw; decorate. Qed.
+
+ Lemma strong_proj_pi2_purerw: forall X Y' Y (f1: term Y X) (f2: term Y' X),
+   PURE f1 -> pi2 o pair f1 f2 == f2.
+ Proof. intros. apply strong_proj_pi2_rorw;decorate. Qed.
+
+ Lemma strong_perm_proj_pi1_rwpure: forall X Y' Y (f1: term Y X) (f2: term Y' X),
+   PURE f2 -> pi1 o perm_pair f1 f2 == f1.
+ Proof.
+     intros. unfold perm_pair. unfold permut. rewrite assoc.
+     remember sc. rewrite strong_proj_pi1_purepure; (solve[decorate] || idtac). 
+     apply strong_proj_pi2_rorw;decorate.
+ Qed.
+
+ Lemma weak_perm_proj_pi2_rwpure: forall X Y' Y (f1: term Y X) (f2: term Y' X),
+   PURE f2 -> pi2 o perm_pair f1 f2 ~~ f2.
+ Proof.
+     intros. unfold perm_pair. unfold permut. rewrite assoc. 
+     remember wsc; rewrite strong_proj_pi2_purepure; (solve[decorate] || idtac). 
+     apply weak_proj_pi1_rorw; decorate.
+ Qed.
+
+(* -------------------- End of Derived Pair Projections -------------------- *)
+
+End Make.
+
