Derived_Rules.v
@@ -1,7 +1,7 @@
 (**************************************************************************)
-(*  This is part of IMP-STATES, it is distributed under the terms of the  *)
-(*              GNU Lesser General Public License version 3               *)
-(*                  (see file LICENSE for more details)                   *)
+(*  This is part of STATES, it is distributed under the terms of the      *)
+(*         GNU Lesser General Public License version 3                    *)
+(*              (see file LICENSE for more details)                       *)
 (*                                                                        *)
 (*       Copyright 2014: Jean-Guillaume Dumas, Dominique Duval            *)
 (*			 Burak Ekici, Damien Pous.                        *)
@@ -9,497 +9,144 @@
 
 Require Import Relations Morphisms.
 Require Import Program.
-Require Memory Terms Decorations Derived_Terms Axioms.
+Require Memory Terms Decorations Derived_Terms Axioms Derived_Pairs Derived_Products.
 Set Implicit Arguments.
-Require Import ZArith.
-Open Scope Z_scope.
 
 Module Make(Import M: Memory.T).
-  Module Export Derived_RulesExp := Axioms.Make(M). 
+  Module Export Derived_RulesExp := Derived_Products.Make(M). 
 
 (* --- Derived Rules --- *)
 
  Lemma weak_refl: forall X Y (f: term Y X), f ~~ f.
- Proof.
-     intros. apply strong_to_weak. apply strong_refl.
- Qed.
+ Proof. intros. apply strong_to_weak. apply strong_refl. Qed.
  
  Lemma zero_weak_to_strong: forall X Y (f g: term Y X),
- is pure f -> is pure g -> f ~~ g  -> f == g.
- Proof.
-     intros. apply one_weak_to_strong.
-     apply is_pure_ro. assumption.
-     apply is_pure_ro. assumption.
-     assumption.
- Qed.
+ PURE f -> PURE g -> f ~~ g  -> f == g.
+ Proof. intros. apply one_weak_to_strong; decorate. Qed.
 
  Lemma weak_final_unit: forall X (f: term unit X), f ~~ forget.
- Proof.
-     intros. remember weak_final_unique.
-     specialize(@weak_final_unique _ f forget).
-     intros. assumption.
- Qed.
+ Proof. intros. apply weak_final_unique. Qed.
 
-Lemma E_1_1: forall X (f g: term unit X),
- is ro f -> is ro g -> f == g.
- Proof.
-     intros. apply one_weak_to_strong.
-     assumption. assumption. 
-     remember weak_final_unique.
-     apply weak_final_unique.
- Qed.
+ Lemma E_1_1: forall X (f g: term unit X), RO f -> RO g -> f == g.
+ Proof. intros. apply one_weak_to_strong; (solve[decorate] || idtac). apply weak_final_unique. Qed.
 
- Lemma E_0_1: forall X (f g : term unit X),
- is pure f -> is pure g -> f == g.
- Proof.
-     intros. apply one_weak_to_strong.
-     apply is_pure_ro. assumption.
-     apply is_pure_ro. assumption.
-     apply weak_final_unique.
- Qed.
+ Lemma E_0_1: forall X (f g : term unit X), PURE f -> PURE g -> f == g.
+ Proof. intros. apply one_weak_to_strong; try decorate. apply weak_final_unique. Qed.
 
- Lemma E_1_2: forall X (f: term unit X), is ro f -> f == forget.
- Proof.
-     intros. apply one_weak_to_strong. assumption.
-     apply is_pure_ro. apply is_forget. 
-     apply weak_final_unique.
- Qed.
+ Lemma E_1_2: forall X (f: term unit X), RO f -> f == forget.
+ Proof. intros. apply one_weak_to_strong; (solve[decorate] || idtac). apply weak_final_unique. Qed.
  
- Lemma E_0_2: forall X (f: term unit X), is pure f -> f == forget.
- Proof.
-     intros. apply one_weak_to_strong. apply is_pure_ro.
-     assumption. apply is_pure_ro.
-     apply is_forget. apply weak_final_unique.
- Qed.
+ Lemma E_0_2: forall X (f: term unit X), PURE f -> f == forget.
+ Proof. intros. apply one_weak_to_strong; (solve[decorate] || idtac). apply weak_final_unique. Qed.
 
  Lemma E_1_3: forall X Y (g: term unit Y) (h: term unit X) 
- (f: term Y X),  is ro g -> is ro h -> is ro f -> h == g o f.
- Proof.
-     intros. apply one_weak_to_strong. assumption.
-     apply is_comp. assumption. assumption.
-     specialize(@weak_final_unique _ h forget).
-     specialize(@weak_final_unique _ (g o f) forget).
-     intros. setoid_rewrite H3 at 1. setoid_rewrite H2 at 1.
-     apply weak_refl.
- Qed.
+ (f: term Y X),  RO g -> RO h -> RO f -> h == g o f.
+ Proof. intros. apply one_weak_to_strong; (solve[decorate] || idtac). apply weak_final_unique. Qed.
 
  Lemma E_0_3: forall X Y (g: term unit Y) (h: term unit X) 
- (f: term Y X), is pure g -> is pure h -> is pure f -> h == g o f.
+ (f: term Y X), PURE g -> PURE h -> PURE f -> h == g o f.
+ Proof. intros. apply one_weak_to_strong; (solve[decorate] || idtac). apply weak_final_unique. Qed.
+
+ Lemma E_1_4: forall X (f: term X unit), RO f -> forget o f == (@id unit).
+ Proof. intros. apply one_weak_to_strong; (solve[decorate] || idtac). apply weak_final_unique. Qed.
+
+ Lemma E_0_4: forall X (f: term X unit), PURE f -> forget o f == (@id unit).
+ Proof. intros. apply one_weak_to_strong; (solve[decorate] || idtac). apply weak_final_unique. Qed.
+
+ Lemma strong_unit_pi1__prod_forget: forall X Y: Type, 
+       forget o pi1 == (@prod_forget X Y).
  Proof.
-     intros. apply one_weak_to_strong. apply is_pure_ro. assumption.
-     apply is_comp. apply is_pure_ro. assumption.
-     apply is_pure_ro. assumption.
-     specialize(@weak_final_unique _ h forget).
-     specialize(@weak_final_unique _ (g o f) forget).
-     intros. setoid_rewrite H3 at 1. setoid_rewrite H2 at 1.
-     apply weak_refl.
+     intros. specialize(@E_0_3 _ _ forget prod_forget (@pi1 X Y)).
+     intros. apply strong_sym. apply H; decorate.
  Qed.
 
- Lemma E_1_4: forall X (f: term X unit), is ro f -> forget o f == (@id unit).
+ Lemma strong_unit_pi2__prod_forget: forall X Y: Type,
+       forget o pi2 == (@prod_forget X Y).
  Proof.
-     intros. apply one_weak_to_strong. apply is_comp. 
-     apply is_pure_ro. apply is_forget.
-     assumption. apply is_pure_ro. apply is_id.
-     remember weak_final_unique.
-     specialize(@weak_final_unique _ (forget o f) forget). intros.
-     specialize(@weak_final_unique _ id forget). intros.
-     setoid_rewrite H0 at 1. setoid_rewrite H1 at 1.
-     apply weak_refl.
+     intros. specialize(@E_0_3 _ _ forget prod_forget (@pi2 X Y)).
+     intros. apply strong_sym. apply H; decorate.
  Qed.
 
- Lemma E_0_4: forall X (f: term X unit),
- is pure f -> forget o f == (@id unit).
- Proof.
-     intros. apply one_weak_to_strong. apply is_comp. 
-     apply is_pure_ro. apply is_forget.
-     apply is_pure_ro. assumption. apply is_pure_ro. apply is_id.
-     specialize(@weak_final_unique _ (forget o f) forget).
-     specialize(@weak_final_unique _ id forget).
-     intros. setoid_rewrite H1 at 1.
-     setoid_rewrite H0 at 1. apply weak_refl.     
- Qed.
+Lemma strong_pi1_inv_pi1__id: forall X: Type, pi1 o inv_pi1 == (@id X).
+ Proof. intros. apply strong_proj_pi1_purepure; decorate. Qed.
 
- Lemma strong_unicity: forall X Y Y'(f g: term (Y/*/Y') X),
+ Lemma strong_pi2_inv_pi1__unit: forall X: Type, pi2 o inv_pi1 == (@forget X).
+ Proof. intros. apply strong_proj_pi2_purepure; decorate. Qed.
+
+ Lemma strong_pi1_permut__pi2: forall X Y: Type, pi1 o permut == (@pi2 X Y).
+ Proof. intros. apply strong_proj_pi1_purepure; decorate. Qed.
+
+ Lemma strong_pi2_permut__pi1: forall X Y: Type, pi2 o permut == (@pi1 X Y).
+ Proof. intros. apply strong_proj_pi2_purepure; decorate. Qed.
+ 
+ Lemma unicity_rect: forall X X' Y Y'(f g: term (Y*Y') (X*X')),
+   (pi1 o f ~~ pi1 o g) -> (pi2 o f ~~ pi2 o g) -> f ~~ g.
+ Proof. intros. apply unicity; assumption. Qed.
+ 
+ Lemma strong_unicity: forall X Y Y'(f g: term (Y*Y') X),
    (pi1 o f ~~ pi1 o g) -> (pi2 o f == pi2 o g) -> f == g.
  Proof.
-     intros.
-     remember comp_final_unique.
-     remember unicity.
-     apply comp_final_unique.
-     transitivity (forget o pi2 o f).
-     apply strong_subs.
-     apply E_0_1. apply is_forget. 
-     apply is_comp.
-     apply is_forget. apply is_pi2.
-     apply strong_sym.
-
-     transitivity (forget o pi2 o g).
-     apply strong_subs.
-     apply E_0_1. apply is_forget.
-     apply is_comp.
-     apply is_forget. apply is_pi2.
-     setoid_rewrite <- assoc at 1.
-     setoid_rewrite <- assoc at 1.
-     
-     apply strong_repl.
-     apply strong_sym. assumption.
-
-     apply unicity.
-     assumption.
-     apply strong_to_weak.
-     assumption.
+     intros. apply comp_final_unique. remember sc.
+     specialize (@E_0_1 _ (forget) (forget o (@pi2 Y Y'))). intros.
+     rewrite H1; (solve[decorate] || idtac). repeat rewrite <- assoc. apply sc. 
+     apply strong_refl. assumption. 
+     apply unicity. assumption. apply strong_to_weak. assumption.
  Qed.
  
- Lemma strong_unicity_rect: forall X X' Y Y'(f g: term (Y/*/Y') (X/*/X')),
+ Lemma strong_perm_unicity: forall X Y Y'(f g: term (Y'*Y) X),
+   (pi1 o f == pi1 o g) -> (pi2 o f ~~ pi2 o g) -> f == g.
+ Proof.
+     intros. apply comp_final_unique. remember sc.
+     specialize (@E_0_1 _ (forget) (forget o (@pi1 Y' Y))). intros.
+     rewrite H1; (solve[decorate] || idtac). repeat rewrite <- assoc. apply sc. 
+     apply strong_refl. assumption. 
+     apply unicity. apply strong_to_weak. assumption. assumption.
+ Qed.
+
+ Lemma strong_unicity_rect: forall X X' Y Y'(f g: term (Y*Y') (X*X')),
    (pi1 o f ~~ pi1 o g) -> (pi2 o f == pi2 o g) -> f == g.
- Proof.
-     intros. remember strong_unicity.
-     specialize (@strong_unicity _ _ _ f g).
-     intros. apply H1. assumption. assumption.
- Qed.
+ Proof. intros. apply strong_unicity; assumption. Qed.
 
- Lemma annihilation_update_lookup: forall i: Loc,
- update i o lookup i == id. (* Prop: 2.1: All Cases *)
- Proof.
-     intros. apply observation. intro k. intros.
-     destruct (Loc_dec i k). rewrite <- e.
-     (*Case k = i*)
-     rewrite assoc.
-     setoid_rewrite -> id_src. setoid_rewrite <- id_tgt at 6.
-     apply weak_subs. apply axiom_1.
-     (*Case k <> i*)
-     rewrite assoc.
-     transitivity (lookup k o forget o lookup i).
-     apply weak_subs. apply axiom_2. assumption.
-     apply strong_to_weak. rewrite <- assoc.
-     apply strong_repl. apply E_1_4. apply is_lookup.
- Qed.
+ Lemma strong_perm_unicity_rect: forall X X' Y Y'(f g: term (Y*Y') (X*X')),
+   (pi1 o f == pi1 o g) -> (pi2 o f ~~ pi2 o g) -> f == g.
+ Proof. intros. apply strong_perm_unicity; assumption. Qed.
 
- Lemma interaction_update_lookup: forall i: Loc,
-  lookup i o update i ~~ id. (* Prop: 2.4: All Cases *)
+ Lemma permuted_pair: forall X Y' Y (f1: term Y X) (f2: term Y' X), 
+  RO f1 -> permut o perm_pair f2 f1 == pair f1 f2.
  Proof.
-     intros. apply axiom_1.
- Qed.
-
- Lemma commutation_lookup_constant: forall i: Loc, forall c: Z, 
- lookup i o update i o (@constant Z c)
- == 
- (@constant Z c) o update i o (@constant Z c). (*Prop 2.8: All Cases*)
- Proof.
-     intros. remember comp_final_unique.
-     specialize (@comp_final_unique _ _
-     ((lookup i o update i) o (@constant Z c)) (((@constant Z c) o update i) o (@constant Z c))).
-     intros. apply H.
-     (* Case 1: <> o f == <> o g *)
-     (*Step 1*)
-     transitivity (update i o (@constant Z c)).
-     setoid_rewrite -> assoc at 1.
-     apply strong_subs.
-     setoid_rewrite -> assoc at 1.
-     setoid_rewrite <- id_tgt at 6.
-     apply strong_subs.
-     remember E_1_4.
-     specialize (@E_1_4 _ (lookup i)).
-     intros. apply H0. apply is_lookup.
-     (*Step 2*)
-     apply strong_sym.
-     setoid_rewrite -> assoc at 1.
-     apply strong_subs.
-     setoid_rewrite <- id_tgt at 6.
-     setoid_rewrite -> assoc at 1.
-     apply strong_subs.
-     remember E_0_4.
-     specialize (@E_0_4 _ (@constant Z c)).
-     intros. apply H0. apply is_constant.
-     (* Case 2: f ~~ g *)
-     (*Step 1*)
-     transitivity ((@constant Z c)).
-     setoid_rewrite <- id_tgt at 6.
-     apply weak_subs. apply axiom_1.
-     (*Step 2*)
-     apply weak_sym.
-     setoid_rewrite <- id_src at 6.
-     setoid_rewrite <- assoc at 1.
-     apply zero_weak_repl. apply is_constant.
-     remember weak_final_unique.
-     specialize (@weak_final_unique _ (update i o (@constant Z c)) (id)).
-     intros. apply H0.
- Qed.
-
- Lemma commutation_update_x_update_y: forall {x y: Loc}, forall (n m: Z), x<>y -> 
-	(update y) o (@constant Z m) o (update x) o (@constant Z n) == 
-        (update x) o (@constant Z n) o (update y) o (@constant Z m).
- Proof.
-    intros. apply observation. intros.
-    (* i = y *)
-    destruct (Loc_dec i y). rewrite e.
-    (*step 1*)
-    transitivity(id o (@constant Z m) o (update x) o (@constant Z n)).
-    rewrite assoc. apply weak_subs. rewrite assoc.
-    apply weak_subs. rewrite assoc.  apply weak_subs.
-    apply axiom_1.
-    (*step 2*)
-    transitivity ((@id Z) o (@constant Z m) o (@id (unit))).
-    rewrite <-assoc. rewrite <- assoc. rewrite <- assoc.
-    apply zero_weak_repl. apply is_id. apply zero_weak_repl.
-    apply is_constant. apply weak_final_unique.
-    apply weak_sym.
-    (*step 3*)
-    transitivity((lookup y) o forget o (@constant Z n) o (update y) o (@constant Z m)).
-    rewrite assoc; apply weak_subs. rewrite assoc; apply weak_subs.
-    rewrite assoc; apply weak_subs. apply axiom_2. assumption.
-    (*step 4*)
-    transitivity((lookup y) o (update y) o (@constant Z m)).
-    apply weak_subs; apply weak_subs. apply strong_to_weak.
-    remember E_0_3.
-    setoid_rewrite <- id_src at 6. rewrite <- assoc.
-    apply strong_repl. specialize(@E_0_3 _ _ forget id (@constant Z n)).
-    intros. apply strong_sym. apply H0. apply is_forget.
-    apply is_id. apply is_constant.
-    (*step 5*)
-    transitivity(id o (@constant Z m)).
-    apply weak_subs. apply axiom_1.
-    rewrite <- assoc. apply zero_weak_repl. auto.
-    setoid_rewrite <- id_src at 1. apply weak_refl.
-    (* i = x *)
-    destruct (Loc_dec i x). rewrite e.
-    (*step 1*)
-    transitivity((lookup x) o forget o (@constant Z m) o (update x) o (@constant Z n)).
-    rewrite assoc. apply weak_subs. rewrite assoc. apply weak_subs.
-    rewrite assoc. apply weak_subs. apply axiom_2.  auto.
-    (*step 2*)
-    transitivity((lookup x) o (update x) o (@constant Z n)).
-    apply weak_subs. apply weak_subs. apply strong_to_weak.
-    setoid_rewrite <- id_src at 6. rewrite <- assoc.
-    apply strong_repl. specialize(@E_0_3 _ _ forget id (@constant Z m)).
-    intros. apply strong_sym. apply H0. apply is_forget.
-    apply is_id. apply is_constant.    
-    (*step 3*)
-    transitivity(id o (@constant Z n)).
-    apply weak_subs. apply axiom_1.
-    apply weak_sym.
-    (*step 4*)
-    transitivity(id o (@constant Z n) o update y o (@constant Z m)).
-    rewrite assoc. apply weak_subs. rewrite assoc.
-    apply weak_subs. rewrite assoc.  apply weak_subs.
-    apply axiom_1.
-    (*step 5*)
-    transitivity ((@id Z) o (@constant Z n) o (@id (unit))).
-    rewrite <-assoc. rewrite <- assoc. rewrite <- assoc.
-    apply zero_weak_repl. apply is_id. apply zero_weak_repl.
-    apply is_constant. apply weak_final_unique.
-    apply weak_sym.
-    rewrite <- assoc. apply zero_weak_repl. auto.
-    setoid_rewrite <- id_src at 1. apply weak_refl.
-    (* i <> x and i <> y *)
-    (*step 1*)
-    transitivity((lookup i) o forget o (@constant Z m) o (update x) o (@constant Z n)).
-    rewrite assoc. apply weak_subs. rewrite assoc. apply weak_subs.
-    rewrite assoc. apply weak_subs. apply axiom_2. auto.
-    (*step 2*)
-    transitivity((lookup i) o (update x) o (@constant Z n)).
-    apply weak_subs. apply weak_subs. apply strong_to_weak.
-    setoid_rewrite <- id_src at 6. rewrite <- assoc.
-    apply strong_repl. specialize(@E_0_3 _ _ forget id (@constant Z m)).
-    intros. apply strong_sym. apply H0. apply is_forget.
-    apply is_id. apply is_constant.
-    (*step 3*)
-    transitivity(lookup i o forget o (@constant Z n)).
-    apply weak_subs. apply axiom_2. auto.
-    (*step 4*)
-    transitivity(lookup i o (@id (unit))).
-    apply strong_to_weak. rewrite <- assoc. apply strong_repl.
-    specialize(@E_0_3 _ _ forget id (@constant Z n)).
-    intros. apply strong_sym. apply H0. apply is_forget.
-    apply is_id. apply is_constant.
-    apply weak_sym.
-    (*step 5*)
-    transitivity((lookup i) o forget o (@constant Z n) o (update y) o (@constant Z m)).
-    rewrite assoc. apply weak_subs. rewrite assoc. apply weak_subs.
-    rewrite assoc. apply weak_subs. apply axiom_2.  auto.
-    (*step 6*)
-    transitivity((lookup i) o (update y) o (@constant Z m)).
-    apply weak_subs. apply weak_subs. apply strong_to_weak.
-    setoid_rewrite <- id_src at 6. rewrite <- assoc.
-    apply strong_repl. specialize(@E_0_3 _ _ forget id (@constant Z n)).
-    intros. apply strong_sym. apply H0. apply is_forget.
-    apply is_id. apply is_constant.
-    (*step 7*)
-    transitivity(lookup i o forget o (@constant Z m)).
-    apply weak_subs. apply axiom_2. auto.
-    apply strong_to_weak. rewrite <- assoc.
-    apply strong_repl. specialize(@E_0_3 _ _ forget id (@constant Z m)).
-    intros. apply strong_sym. apply H0. apply is_forget.
-    apply is_id. apply is_constant.
+     intros. apply strong_unicity. rewrite assoc. remember wsc.
+     rewrite strong_pi1_permut__pi2. rewrite weak_perm_proj_pi2_rwro; (solve[decorate] || idtac).
+     apply weak_sym. apply weak_proj_pi1_rorw; decorate.
+     rewrite assoc. remember sc. rewrite strong_pi2_permut__pi1.
+     rewrite strong_perm_proj_pi1_rwro; (solve[decorate] || idtac). apply strong_sym.
+     apply strong_proj_pi2_rorw; decorate.
  Qed. 
 
-
- Lemma pair_ex: forall (m: Loc) (c0 c1: Z),
-       gt o (pair (lookup m) (constant c1)) o update m o constant c0
-	~~
-       gt o (pair (constant c0) (constant c1)).  
+ Lemma obs_local_global_2: forall X Y (f g : term Y X),
+ (forall i: Loc, lookup i o forget o f ~~ lookup i o forget o g) ->  f ~~ g -> f == g.
  Proof.
-     intros. rewrite <- assoc. rewrite <- assoc.
-     apply zero_weak_repl. auto. apply unicity.
-     transitivity((lookup m) o (update m o constant c0)).
-     rewrite assoc. apply weak_subs.
-     apply weak_proj_pi1_rorw. auto.
-     transitivity(id o constant c0). rewrite assoc.
-     apply weak_subs. apply axiom_1. rewrite id_tgt.
-     apply weak_sym. apply weak_proj_pi1_rorw. auto.
-     transitivity(constant c1 o update m o constant c0).
-     rewrite assoc. rewrite assoc. apply weak_subs.
-     apply weak_subs. apply strong_to_weak.
-     apply strong_proj_pi2_rorw. auto.
-     transitivity(constant c1 o forget o constant c0).
-     apply weak_subs. apply zero_weak_repl.
-     auto. apply weak_final_unique.
-     transitivity(constant c1 o id). rewrite <- assoc.
-     apply zero_weak_repl. auto. apply weak_final_unique.
-     rewrite id_src. apply weak_sym. apply strong_to_weak.
-     apply strong_proj_pi2_rorw. auto.     
+     intros. apply comp_final_unique. apply observation. intros.
+     rewrite assoc. rewrite assoc. apply H. assumption.
  Qed.
 
- Lemma pair_ex_2: forall (m n: Loc) (c0 c1: Z),
-       gt o (pair (lookup m) (constant c1)) o update m o constant c0 o update n o constant c1 
-	~~
-       gt o (pair (constant c0) (constant c1)).  
+ (* additional lemmas about [passbool] and [copair] *)
+ Lemma passbool_true: passbool o constant true == copi1.
  Proof.
-     intros. rewrite <- assoc. rewrite <- assoc.
-     rewrite <- assoc. rewrite <- assoc.
-     apply zero_weak_repl. auto. apply unicity.
-     transitivity((lookup m) o (update m o constant c0) o (update n o constant c1)).
-     rewrite assoc. rewrite assoc. rewrite assoc. apply weak_subs.
-     rewrite <- assoc. apply weak_subs. apply weak_proj_pi1_rorw. auto.
-     transitivity(id o constant c0 o update n o constant c1).
-     rewrite assoc. apply weak_subs. apply weak_subs. 
-     rewrite assoc. apply weak_subs. apply axiom_1.
-     transitivity(id o constant c0 o forget o constant c1).
-     rewrite <- assoc. rewrite <- assoc. rewrite <- assoc.
-     rewrite <- assoc. apply zero_weak_repl. auto.
-     apply zero_weak_repl. auto. apply weak_final_unique.
-     transitivity(id o constant c0 o id). rewrite <- assoc.
-     apply zero_weak_repl. auto. apply weak_final_unique.
-     rewrite id_src. rewrite id_tgt. apply weak_sym. 
-     apply weak_proj_pi1_rorw. auto. 
-     transitivity(constant c1 o update m o constant c0 o update n o constant c1).
-     rewrite <- assoc.  rewrite <- assoc.  rewrite <- assoc. 
-     rewrite assoc. apply weak_subs. apply strong_to_weak.
-     apply strong_proj_pi2_rorw. auto.
-     transitivity((((constant c1 o forget) o constant c0) o update n) o constant c1).
-     apply weak_subs. apply weak_subs. apply weak_subs. 
-     apply zero_weak_repl. auto. apply weak_final_unique.
-     transitivity(constant c1 o forget o (constant c0) o forget o constant c1).
-     apply weak_subs. apply zero_weak_repl. auto. apply weak_final_unique.
-     transitivity((((constant c1 o forget) o constant c0) o id)).
-     rewrite <- assoc. apply zero_weak_repl. auto. apply weak_final_unique.
-     transitivity(constant c1 o id o id). apply weak_subs.
-     rewrite <- assoc. apply zero_weak_repl. auto. apply weak_final_unique.
-     rewrite id_src. rewrite id_src. apply weak_sym. apply strong_to_weak.
-     apply strong_proj_pi2_rorw. auto.     
- Qed.     
- 
-
- Lemma strong_pair: forall (m: Loc) (p q: Z),
-      (pair (lookup m) (constant q)) o update m o constant p
-      ==
-      (pair (constant p) (constant q)) o update m o constant p.
- Proof.
-      intros. apply strong_unicity.
-      transitivity(lookup m o update m o constant p).
-      rewrite assoc. apply weak_subs. rewrite assoc.
-      apply weak_subs. apply weak_proj_pi1_rorw. auto.
-      transitivity(id o constant p).
-      apply weak_subs. apply axiom_1. apply weak_sym.
-      transitivity(constant p o update m o constant p).
-      rewrite assoc. apply weak_subs. rewrite assoc.
-      apply weak_subs. apply weak_proj_pi1_rorw. auto.
-      rewrite id_tgt. setoid_rewrite <- id_src at 6.
-      rewrite <- assoc. apply zero_weak_repl. auto.
-      apply weak_final_unique.
-      transitivity(constant q o update m o constant p).
-      rewrite assoc. apply strong_subs. rewrite assoc.
-      apply strong_subs. apply strong_proj_pi2_rorw. auto.
-      apply strong_sym.
-      transitivity(constant q o update m o constant p).
-      rewrite assoc. apply strong_subs. rewrite assoc.
-      apply strong_subs. apply strong_proj_pi2_rorw. auto.
-      apply strong_refl.      
+     unfold passbool. unfold constant. rewrite pure_pure. unfold copi1.
+     apply pure_eq. intros. simpl. rewrite x. reflexivity.
  Qed.
 
- Lemma perm_strong_pair: forall (m: Loc) (p q: Z),
-      (pair (constant q) (lookup m)) o update m o constant p
-      ==
-      (pair (constant q) (constant p)) o update m o constant p.
- Proof.
-      intros. apply strong_unicity.
-      transitivity(constant q o update m o constant p).
-      rewrite assoc. apply weak_subs. rewrite assoc.
-      apply weak_subs. apply weak_proj_pi1_rorw. auto.
-      apply weak_sym. rewrite assoc. apply weak_subs.
-      rewrite assoc. apply weak_subs. 
-      apply weak_proj_pi1_rorw. auto.
-      transitivity(lookup m o update m o constant p).
-      rewrite assoc. apply strong_subs. rewrite assoc.
-      apply strong_subs. apply strong_proj_pi2_rorw. auto.
-      transitivity(constant p o update m o constant p).
-      specialize(@commutation_lookup_constant m p). intros.
-      apply H. apply strong_sym. rewrite assoc. apply strong_subs.
-      rewrite assoc. apply strong_subs.
-      apply strong_proj_pi2_rorw. auto.
+ Lemma passbool_false: passbool o constant false == copi2.
+ Proof. 
+    unfold passbool. unfold constant. setoid_rewrite pure_pure.
+    apply pure_eq.  now intros [].
  Qed.
 
- Lemma or_ex1: orB o (pair (le o (pair (@constant Z 80) (@constant Z 80)))
- (lt o (pair (@constant Z 180) (@constant Z 80))))
-       == 
-      ttrue.
- Proof.
-    apply IMP_IntOrT. left.
-    transitivity((le o pair (constant 80) (constant 80))).
-    apply one_weak_to_strong. auto. apply is_comp. auto.
-    apply is_pair. auto. auto. auto.
-    apply weak_proj_pi1_rorw. auto.
-    apply IMP_IntLeT. simpl. auto.
- Qed.
+ Lemma copair_true A f g: @copair _ _ A f g o (passbool o constant true) == f.
+ Proof. rewrite passbool_true. apply strong_coproj_copi1_rwrw. Qed.
 
- Lemma or_ex2: orB o (pair (lt o (pair (@constant Z 80) (@constant Z 80)))
- (lt o (pair (@constant Z 180) (@constant Z 80))))
-       == 
-      ffalse.
- Proof.
-    apply IMP_IntOrF. 
-    transitivity((lt o pair (constant 80) (constant 80))).
-    apply one_weak_to_strong. auto. apply is_comp. auto.
-    apply is_pair. auto. auto. auto.
-    apply weak_proj_pi1_rorw. auto. apply IMP_IntLtF. simpl. auto.
-    transitivity((lt o pair (constant 180) (constant 80))).
-    apply strong_proj_pi2_rorw. auto. apply IMP_IntLtF. simpl. auto.
- Qed.
-
- Lemma and_ex1: andB o (pair (le o (pair (@constant Z 80) (@constant Z 80)))
- (lt o (pair (@constant Z 180) (@constant Z 80))))
-       == 
-      ffalse.
- Proof.
-    apply IMP_IntAndF. right.
-    transitivity((lt o pair (constant 180) (constant 80))).
-    apply strong_proj_pi2_rorw. auto. apply IMP_IntLtF. simpl. auto.
- Qed.
-
- Lemma and_ex2: andB o (pair (le o (pair (@constant Z 80) (@constant Z 80)))
- (gt o (pair (@constant Z 180) (@constant Z 80))))
-       == 
-      ttrue.
- Proof.
-    apply IMP_IntAndT. 
-    transitivity((le o pair (constant 80) (constant 80))).
-    apply one_weak_to_strong. auto. apply is_comp. auto.
-    apply is_pair. auto. auto. auto.
-    apply weak_proj_pi1_rorw. auto.
-    apply IMP_IntLeT. simpl. auto.
-    transitivity((gt o pair (constant 180) (constant 80))).
-    apply strong_proj_pi2_rorw. auto. apply IMP_IntGtT. simpl. auto.
- Qed.
+ Lemma copair_false A f g: @copair _ _ A f g o (passbool o constant false) == g.
+ Proof. rewrite passbool_false. apply strong_coproj_copi2_rwrw. Qed.
 
 (* -------------------- End of Derived Rules -------------------- *)
 
