IMP_Proofs.v
@@ -9,964 +9,159 @@
 
 Require Import Relations Morphisms.
 Require Import Program.
-Require Memory Terms Decorations Derived_Terms Axioms
-Derived_Rules IMP_to_COQ.
+Require Memory Terms Decorations Axioms Derived_Terms Derived_Pairs
+        Derived_Products Derived_Rules Proofs IMP_to_COQ.
 Set Implicit Arguments.
 Require Import ZArith.
+Require Import Bool.
 Open Scope Z_scope.
 
 Module Make(Import M: Memory.T).
-  Module Export ConversionExp := IMP_to_COQ.Make(M).
+  Module Export IMP_ProofsExp := IMP_to_COQ.Make(M).
 
  Lemma IMP_ex1: forall (x y: Loc) (p q: Z), x <> y ->
-      {{x ::= (const p) ;; 
-        y ::= (const q)}}
-      ==
-      {{y ::= (const q);; 
-        x ::= (const p)}}.
- Proof.
-   intros. unfold defCommand. unfold defArithExp.
-   remember (@commutation_update_x_update_y y x).
-   specialize(@commutation_update_x_update_y y x q p). intros.
-   rewrite assoc. rewrite assoc. apply strong_sym.
-   apply H0. auto.
- Qed.
+   {{x ::= const p ;; (y ::= const q)}} 
+   ==
+   {{y ::= const q ;;  (x ::= const p)}}.
+ Proof. intros. simpl. now apply commutation_update_update. Qed.
 
- Lemma IMP_ex2: forall m: Loc,
-       {{IFB (constT ttrue) 
+ Lemma IMP_ex2: forall (m: Loc),
+       {{IFB (const true) 
            THEN (m ::= const (-30)) 
          ELSE (SKIP)
          ENDIF}}
        ==
-       {{IFB (constF ffalse) 
+       {{IFB (const false) 
            THEN (SKIP) 
          ELSE (m ::= const (-30))
          ENDIF}}.
- Proof.
- intros. simpl.
- transitivity(update m o constant (-30)) .
- apply strong_coproj_copi1_rwrw. apply strong_sym.
- transitivity(update m o constant (-30)). 
- apply strong_coproj_copi2_rwrw. apply strong_refl.
- Qed.
-
+ Proof. intros. simpl. now rewrite copair_true, copair_false. Qed.
 
  Lemma IMP_ex3: forall (x: Loc) (p q: Z),
       {{x ::= (const p)  ;;
-        x ::= (const q)}}
+        (x ::= (const q))}}
       ==
       {{x ::= (const q)}}.
  Proof.
-     intros. simpl.
-     apply observation. intros. destruct(Loc_dec i x). rewrite e.
-     transitivity(lookup x o update x o constant q o 
-     (forget o constant p)).
-     transitivity(id o constant q o update x o constant p).
-     rewrite assoc. rewrite assoc. apply weak_subs. apply weak_subs.
-     rewrite assoc. apply weak_subs. apply axiom_1.
-     apply weak_sym.
-     transitivity(id o constant q o forget o constant p).
-     rewrite assoc. apply weak_subs. apply weak_subs. apply weak_subs.
-     apply axiom_1. 
-     rewrite <- assoc. rewrite <- assoc. 
-     rewrite <- assoc. rewrite <- assoc.
-     apply zero_weak_repl. auto. apply zero_weak_repl. auto. 
+     intros. simpl. apply observation. intros. destruct(Loc_dec i x). rewrite e.
+     repeat rewrite assoc. rewrite axiom_1. setoid_rewrite id_tgt.
+     setoid_rewrite <- id_src at 6. rewrite <- assoc. apply wrc; try decorate.
      apply weak_final_unique.
-     transitivity(id o constant q o forget o constant p).
-     rewrite assoc. apply weak_subs. apply weak_subs.
-     apply weak_subs. apply axiom_1.
-     transitivity(id o constant q o id). rewrite <- assoc.
-     apply zero_weak_repl. auto. apply weak_final_unique.
-     apply weak_sym.
-     transitivity(id o constant q).
-     rewrite assoc. apply weak_subs. apply axiom_1.
-     rewrite <- assoc. apply zero_weak_repl. auto.
-     rewrite id_src. apply weak_refl.
-     transitivity(lookup i o forget o constant q o update x o constant p).
-     rewrite assoc. rewrite assoc. apply weak_subs. apply weak_subs.
-     rewrite assoc. apply weak_subs. apply axiom_2. auto.
-     transitivity(lookup i o id o update x o constant p).
-     apply weak_subs. apply weak_subs. apply strong_to_weak. 
-     rewrite <- assoc. apply strong_repl. apply zero_weak_to_strong.
-     auto. auto. apply weak_final_unique.
-     transitivity(lookup i o forget o constant p).
-     apply weak_subs.
-     transitivity(lookup i o update x).
-     apply weak_subs. rewrite id_src. apply weak_refl.
-     apply axiom_2. auto.
-     transitivity(lookup i o id). apply strong_to_weak.
-     rewrite <- assoc. apply strong_repl. apply zero_weak_to_strong.
-     auto. auto. apply weak_final_unique. apply weak_sym.
-     transitivity(lookup i o forget o constant q).
-     rewrite assoc. apply weak_subs. apply axiom_2. auto.
-     apply strong_to_weak. rewrite <- assoc. apply strong_repl.
-     apply zero_weak_to_strong. auto. auto. apply weak_final_unique.  
+     repeat rewrite assoc. rewrite axiom_2; try auto. specialize(@E_0_4 _ (constant q)). 
+     intros. setoid_rewrite <- assoc at 3. rewrite H; try decorate. rewrite id_src.
+     rewrite axiom_2; auto. repeat rewrite <- assoc. apply strong_to_weak. 
+     apply sc; try reflexivity. apply zero_weak_to_strong; try decorate.
+     apply weak_final_unique.
  Qed.
 
  Lemma IMP_ex4: forall (x: Loc) (p q: Z),
       {{x ::= (const p)  ;;
-        x ::= (loc x +++ const q)}}
+        (x ::= (loc x +++ const q))}}
       ==
       {{x ::= (const (p+q))}}.
  Proof.
-     intros. simpl.
-     transitivity(update x o (plus o pair (constant p) (constant q)) o 
-     (update x o constant p)). rewrite <- assoc.
-     setoid_rewrite <- assoc at 2. apply strong_repl.
-     rewrite <- assoc. setoid_rewrite <- assoc at 1.
-     apply strong_repl. apply strong_unicity.
-     transitivity(lookup x o update x o constant p).
-     rewrite assoc. rewrite assoc. apply weak_subs. apply weak_subs.
-     apply weak_proj_pi1_rorw. auto. apply weak_sym.
-     apply strong_to_weak. 
-     transitivity(constant p o update x o constant p).
-     rewrite assoc. rewrite assoc. apply strong_subs. apply strong_subs.
-     apply one_weak_to_strong. auto. auto.
-     apply weak_proj_pi1_rorw. auto.
-     remember commutation_lookup_constant.
-     specialize(@commutation_lookup_constant x p). intros.
-     apply strong_sym. apply H.
-     transitivity(constant q o update x o constant p).
-     rewrite assoc. rewrite assoc. apply strong_subs. apply strong_subs.
-     apply strong_proj_pi2_rorw. auto. apply strong_sym.
-     transitivity(constant q o update x o constant p).
-     rewrite assoc. rewrite assoc. apply strong_subs. apply strong_subs.
-     apply strong_proj_pi2_rorw. auto. apply strong_refl.
-     transitivity((update x o constant (p+q) o (update x o constant p))).
-     apply strong_subs. apply strong_repl. apply IMP_IntAdd.
-     
-     remember IMP_ex3.
-     specialize(@IMP_ex3 x p (p+q)). intros. simpl in H. apply H.
+ intros. simpl. do 2 setoid_rewrite <- assoc at 1.
+ rewrite commutation_lookup_constant_update. setoid_rewrite assoc at 2.
+ rewrite IMP_IntAdd. rewrite assoc. rewrite (@IMP_ex3 x p (add(p,q))). reflexivity. 
  Qed.
 
- Lemma IMP_ex5: forall (x: Loc) (p q: Z),
-      {{x ::= (const p)  ;;
-        x ::= (loc x *** const q)}}
-      ==
-      {{x ::= (const (p*q))}}.
- Proof.
-     intros. simpl.
-     transitivity(update x o (mult o pair (constant p) (constant q)) o 
-     (update x o constant p)). rewrite <- assoc.
-     setoid_rewrite <- assoc at 2. apply strong_repl.
-     rewrite <- assoc. setoid_rewrite <- assoc at 1.
-     apply strong_repl. apply strong_unicity.
-     transitivity(lookup x o update x o constant p).
-     rewrite assoc. rewrite assoc. apply weak_subs. apply weak_subs.
-     apply weak_proj_pi1_rorw. auto. apply weak_sym.
-     apply strong_to_weak. 
-     transitivity(constant p o update x o constant p).
-     rewrite assoc. rewrite assoc. apply strong_subs. apply strong_subs.
-     apply one_weak_to_strong. auto. auto.
-     apply weak_proj_pi1_rorw. auto.
-     remember commutation_lookup_constant.
-     specialize(@commutation_lookup_constant x p). intros.
-     apply strong_sym. apply H.
-     transitivity(constant q o update x o constant p).
-     rewrite assoc. rewrite assoc. apply strong_subs. apply strong_subs.
-     apply strong_proj_pi2_rorw. auto. apply strong_sym.
-     transitivity(constant q o update x o constant p).
-     rewrite assoc. rewrite assoc. apply strong_subs. apply strong_subs.
-     apply strong_proj_pi2_rorw. auto. apply strong_refl.
-     transitivity((update x o constant (p*q) o (update x o constant p))).
-     apply strong_subs. apply strong_repl. apply IMP_IntMult.
-     
-     remember IMP_ex3.
-     specialize(@IMP_ex3 x p (p*q)). intros. simpl in H. apply H.
- Qed.
-
- Lemma IMP_ex6: forall (x: Loc),
-      {{WHILE (constF ffalse) 
-          DO (x ::= (const 2))
-	ENDWHILE ;; 
-        SKIP}}
-      ==
-      {{SKIP}}.
- Proof.
-     intros. unfold defCommand. unfold defArithExp.
-     unfold defBoolExp. rewrite id_tgt.
-     apply strong_coproj_copi2_rwrw.
- Qed.
-
- Lemma IMP_ex7: forall (x: Loc),
+ Lemma IMP_ex5: forall (x: Loc),
       {{x ::= (const 10) ;;
-        IFB ((loc x) >> (const 5)) 
+        IFB (loc x >> const 5) 
           THEN (x ::= (const 2)) 
         ELSE SKIP 
         ENDIF}}
       ==
       {{x ::= (const 2)}}.
  Proof.
-    intros.  unfold defCommand. unfold defBoolExp. 
-    unfold defArithExp. 
-    transitivity((copair (update x o constant 2) id o
-    (gt o pair (constant 10) (constant 5))) o (update x o constant 10)).
-    rewrite <- assoc. rewrite <- assoc. apply strong_repl. 
-    rewrite <- assoc. rewrite <- assoc. apply strong_repl.
-    specialize(@strong_pair x 10 5). intros. rewrite assoc. 
-    rewrite assoc. apply H. 
-    transitivity((copair (update x o constant 2) id) o ttrue 
-    o (update x o constant 10)).
-    rewrite <- assoc. rewrite <- assoc.
-    apply strong_repl. apply strong_subs. apply IMP_IntGtT. simpl. auto.
-    transitivity((update x o constant 2) o (update x o constant 10)).
-    apply strong_subs. apply strong_coproj_copi1_rwrw.
-    specialize(@IMP_ex3 x 10 2). unfold defCommand.
-    unfold defBoolExp. unfold defArithExp. intros. apply H.   
+    intros. simpl. do 2 setoid_rewrite assoc at 2. setoid_rewrite <- assoc.
+    rewrite commutation_lookup_constant_update. do 2 setoid_rewrite <- assoc at 1.
+    do 2 setoid_rewrite assoc at 2. rewrite IMP_IntGtT by constructor. rewrite assoc.
+    rewrite strong_coproj_copi1_rwrw. rewrite (@IMP_ex3 x 10 2). reflexivity.
  Qed.
 
- Lemma IMP_ex8: forall (x: Loc),
-      {{x ::= (const 10) ;;
-        IFB ((loc x) >>= (const 5))
-          THEN (x ::= (const 2)) 
-        ELSE SKIP 
+ Lemma IMP_condEx: forall (b: bool) (f g: Command),
+      {{IFB const b 
+          THEN (IFB const b THEN f ELSE g ENDIF) 
+        ELSE g 
         ENDIF}}
       ==
-      {{x ::= (const 2)}}.
- Proof.
-    intros.  unfold defCommand. unfold defBoolExp. 
-    unfold defArithExp. 
-    transitivity((copair (update x o constant 2) id o
-    (ge o pair (constant 10) (constant 5))) o (update x o constant 10)).
-    rewrite <- assoc. rewrite <- assoc. apply strong_repl. 
-    rewrite <- assoc. rewrite <- assoc. apply strong_repl.
-    specialize(@strong_pair x 10 5). intros. rewrite assoc. 
-    rewrite assoc. apply H. 
-    transitivity((copair (update x o constant 2) id) o ttrue 
-    o (update x o constant 10)).
-    rewrite <- assoc. rewrite <- assoc.
-    apply strong_repl. apply strong_subs. apply IMP_IntGeT. simpl. auto.
-    transitivity((update x o constant 2) o (update x o constant 10)).
-    apply strong_subs. apply strong_coproj_copi1_rwrw.
-    specialize(@IMP_ex3 x 10 2). unfold defCommand.
-    unfold defBoolExp. unfold defArithExp. intros. apply H.   
- Qed.
-
- Lemma IMP_ex9: forall (x: Loc) (p: Z),
-      {{x ::= (const 10) ;;
-        IFB ((loc x) >>= (const 0))
-          THEN (SKIP) 
-        ELSE (x ::= (loc x *** (const (-1)))) 
-        ENDIF}}
-      ==
-      {{x ::= (const 10) ;;
-        IFB ((loc x) <<= (const 0))
-          THEN (x ::= (loc x *** (const (-1)))) 
-        ELSE (SKIP) 
+      {{IFB const b 
+          THEN f 
+        ELSE g 
         ENDIF}}.
  Proof.
-    intros. unfold defCommand. unfold defBoolExp. 
-    unfold defArithExp.
-    transitivity((copair id (update x o (mult o 
-    pair (lookup x) (constant (-1)))) o 
-    (ge o pair (constant 10) (constant 0))) o 
-    (update x o constant 10)).
-    rewrite <- assoc. rewrite <- assoc. apply strong_repl.
-    rewrite <- assoc. rewrite <- assoc. apply strong_repl.
-    specialize(@strong_pair x 10 0). intros. rewrite assoc. 
-    rewrite assoc. apply H.   
-    transitivity((copair id (update x o (mult o 
-    pair (lookup x) (constant (-1)))) o 
-    (ttrue) o (update x o constant 10))).
-    apply strong_subs. apply strong_repl.
-    apply IMP_IntGeT. simpl. auto.
-    transitivity(id o update x o constant 10).
-    rewrite assoc. apply strong_subs. apply strong_subs.
-    apply strong_coproj_copi1_rwrw. apply strong_sym.
-    transitivity((copair (update x o (mult o 
-    pair (lookup x) (constant (-1)))) id o 
-    (le o pair (constant 10) (constant 0))) o 
-    (update x o constant 10)).
-    rewrite <- assoc. rewrite <- assoc. apply strong_repl.
-    rewrite <- assoc. rewrite <- assoc. apply strong_repl.
-    specialize(@strong_pair x 10 0). intros. 
-    rewrite assoc. rewrite assoc. apply H.
-    transitivity((copair (update x o (mult o 
-    pair (lookup x) (constant (-1)))) id o 
-    (ffalse) o (update x o constant 10))).
-    apply strong_subs. apply strong_repl.
-    apply IMP_IntLeF. simpl. auto.
-    rewrite assoc. apply strong_subs. apply strong_subs.
-    apply strong_coproj_copi2_rwrw.    
- Qed.
-
- Lemma IMP_ex10: forall (x: Loc) (p: Z),
-      {{x ::= (const (-10)) ;;
-        IFB ((loc x) >>= (const 0)) 
-          THEN (SKIP) 
-        ELSE (x ::= (loc x *** (const (-1)))) 
-        ENDIF}}
-      ==
-      {{x ::= (const (-10)) ;;
-        IFB ((loc x) <<= (const 0)) 
-          THEN (x ::= ( loc x *** (const (-1)))) 
-        ELSE (SKIP) 
-        ENDIF}}.
- Proof.
-    intros. unfold defCommand. unfold defBoolExp. 
-    unfold defArithExp.
-    transitivity((copair id (update x o (mult o 
-    pair (lookup x) (constant (-1)))) o 
-    (ge o pair (constant (-10)) (constant 0))) o 
-    (update x o constant (-10))).
-    rewrite <- assoc. rewrite <- assoc. apply strong_repl.
-    rewrite <- assoc. rewrite <- assoc. apply strong_repl.
-    specialize(@strong_pair x (-10) 0). intros. rewrite assoc. 
-    rewrite assoc. apply H.   
-    transitivity((copair id (update x o (mult o 
-    pair (lookup x) (constant (-1)))) o 
-    (ffalse) o (update x o constant (-10)))).
-    apply strong_subs. apply strong_repl.
-    apply IMP_IntGeF. simpl. auto.
-    transitivity((update x o (mult o pair  (lookup x) (constant (-1)))
-    o (update x o constant (-10)))).
-    apply strong_subs. apply strong_coproj_copi2_rwrw.
-    transitivity(update x o mult o 
-    pair (constant (-10)) (constant (-1))
-    o update x o (constant (-10))). apply strong_sym.
-    rewrite <- assoc. rewrite <- assoc.
-    rewrite <- assoc. rewrite <- assoc. apply strong_repl.
-    rewrite <- assoc. apply strong_repl. apply strong_unicity.
-    apply weak_sym.
-    transitivity(lookup x o update x o (constant (-10))).
-    rewrite assoc. rewrite assoc. apply weak_subs. apply weak_subs.
-    apply weak_proj_pi1_rorw. auto.
-    transitivity(id o (constant (-10))). apply weak_subs. apply axiom_1.
-    apply weak_sym.
-    transitivity((constant (-10)) o (update x o constant (-10))).
-    rewrite assoc. apply weak_subs. apply weak_proj_pi1_rorw. auto.
-    transitivity((constant (-10)) o id). apply zero_weak_repl. auto.
-    apply weak_final_unique. rewrite id_tgt. rewrite id_src. apply weak_refl.
-    
-    transitivity((constant (-1)) o update x o (constant (-10))).
-    rewrite assoc. rewrite assoc. apply strong_subs. apply strong_subs.
-    apply strong_proj_pi2_rorw. auto. apply strong_sym.
-    transitivity((constant (-1)) o update x o (constant (-10))).
-    rewrite assoc. rewrite assoc. apply strong_subs. apply strong_subs.
-    apply strong_proj_pi2_rorw. auto. apply strong_refl.
-    transitivity(update x o (constant 10) o update x o (constant (-10))).
-    apply strong_subs. apply strong_subs. rewrite <- assoc.
-    apply strong_repl. apply IMP_IntMult.
-    transitivity(update x o constant 10).
-    specialize(@IMP_ex3 x (-10) 10). unfold defCommand. unfold defBoolExp. 
-    unfold defArithExp. intros. rewrite <- assoc. apply H. apply strong_sym.
-
-    transitivity((copair (update x o (mult o 
-    pair (lookup x) (constant (-1)))) id o 
-    (le o pair (constant (-10)) (constant 0))) o 
-    (update x o constant (-10))).
-    rewrite <- assoc. rewrite <- assoc. apply strong_repl.
-    rewrite <- assoc. rewrite <- assoc. apply strong_repl.
-    specialize(@strong_pair x (-10) 0). intros.
-    rewrite assoc. rewrite assoc. apply H.
-    transitivity((copair (update x o (mult o 
-    pair (lookup x) (constant (-1)))) id o 
-    (ttrue) o (update x o constant (-10)))).
-    apply strong_subs. apply strong_repl. apply IMP_IntLeT.
-    simpl. auto.
-    transitivity((update x o (mult o pair (lookup x) (constant (-1))) o 
-    (update x o constant (-10)))).
-    apply strong_subs. apply strong_coproj_copi1_rwrw.
-    transitivity(update x o mult o pair (constant (-10)) (constant (-1)) o 
-    update x o (constant (-10))). apply strong_sym. rewrite <- assoc.
-    rewrite <- assoc. rewrite <- assoc. rewrite <- assoc. apply strong_repl.
-    rewrite <- assoc. apply strong_repl. apply strong_sym.
-    specialize(@strong_pair x (-10) (-1)). intros. rewrite assoc.
-    rewrite assoc. apply H.
-    transitivity(update x o (constant 10) o update x o (constant (-10))).
-    apply strong_subs. apply strong_subs. rewrite <- assoc. 
-    apply strong_repl. apply IMP_IntMult.  
-    specialize(@IMP_ex3 x (-10) 10). unfold defCommand. unfold defBoolExp. 
-    unfold defArithExp. intros. rewrite <- assoc. apply H. 
- Qed.
-
- Lemma IMP_ex11: forall (x: Loc) (p: Z),
-      {{x ::= (const 0) ;;
-        IFB ((loc x) >>= (const 0)) 
-          THEN (SKIP) 
-        ELSE (x ::= (loc x *** (const (-1)))) 
-        ENDIF}}
-      ==
-      {{x ::= (const 0) ;;
-        IFB ((loc x) <<= (const 0))
-          THEN (x ::= ( loc x *** (const (-1)))) 
-        ELSE (SKIP) 
-        ENDIF}}.
- Proof.
-    intros. unfold defCommand. unfold defBoolExp. 
-    unfold defArithExp.
-    transitivity((copair id (update x o 
-    (mult o pair (lookup x) (constant (-1)))) o 
-    (ge o pair (constant 0) (constant 0))) o (update x o constant 0)).
-    rewrite <- assoc. rewrite <- assoc. apply strong_repl.
-    rewrite <- assoc. rewrite <- assoc. apply strong_repl.
-    specialize(@strong_pair x 0 0). intros.
-    rewrite assoc. rewrite assoc. apply H.
-    transitivity((copair id (update x o 
-    (mult o pair (lookup x) (constant (-1)))) o 
-    (ttrue) o (update x o constant 0))).
-    apply strong_subs. apply strong_repl.
-    apply IMP_IntGeT. simpl. auto.
-    transitivity(id o update x o constant 0).
-    rewrite assoc. apply strong_subs. apply strong_subs.
-    apply strong_coproj_copi1_rwrw. rewrite <- assoc.
-    rewrite id_tgt. apply strong_sym.
-
-    transitivity((copair (update x o 
-    (mult o pair (lookup x) (constant (-1)))) id o 
-    (le o pair (constant 0) (constant 0))) o (update x o constant 0)).
-    rewrite <- assoc. rewrite <- assoc. apply strong_repl.
-    rewrite <- assoc. rewrite <- assoc. apply strong_repl.
-    specialize(@strong_pair x 0 0). intros.
-    rewrite assoc. rewrite assoc. apply H.
-    transitivity((copair (update x o 
-    (mult o pair (lookup x) (constant (-1)))) id o 
-    (ttrue) o (update x o constant 0))).
-    apply strong_subs. apply strong_repl.
-    apply IMP_IntLeT. simpl. auto.
-    transitivity((update x o (mult o pair (lookup x) (constant (-1))))
-    o update x o constant 0).
-    rewrite assoc. apply strong_subs. apply strong_subs.
-    apply strong_coproj_copi1_rwrw.
-    transitivity(update x o mult o pair (constant 0) (constant (-1)) 
-    o update x o constant 0 ). apply strong_sym.
-    rewrite <- assoc. rewrite <- assoc. rewrite <- assoc. 
-    rewrite <- assoc. rewrite <- assoc. apply strong_repl.
-    rewrite <- assoc. apply strong_repl. apply strong_sym.
-    specialize(@strong_pair x 0 (-1)). intros.
-    rewrite assoc. rewrite assoc. apply H.
-    transitivity(update x o (constant 0) o update x o (constant 0)).
-    apply strong_subs. apply strong_subs. rewrite <- assoc.
-    apply strong_repl. apply IMP_IntMult.
-    specialize(@IMP_ex3 x 0 0). unfold defCommand. unfold defBoolExp. 
-    unfold defArithExp. intros. rewrite <- assoc. apply H. 
- Qed.
-
- Lemma IMP_perm_ex11: forall (x: Loc) (p: Z),
-      {{x ::= (const 0) ;;
-        IFB ((loc x) >>= (const 0)) 
-          THEN (SKIP) 
-        ELSE (x ::= ((const (-1)) *** loc x)) 
-        ENDIF}}
-      ==
-      {{x ::= (const 0) ;;
-        IFB ((loc x) <<= (const 0))
-          THEN (x ::= ((const (-1)) *** loc x)) 
-        ELSE (SKIP) 
-        ENDIF}}.
- Proof.
-    intros. unfold defCommand. unfold defBoolExp. 
-    unfold defArithExp.
-    transitivity((copair id (update x o 
-    (mult o pair (constant (-1)) (lookup x))) o 
-    (ge o pair (constant 0) (constant 0))) o (update x o constant 0)).
-    rewrite <- assoc. rewrite <- assoc. apply strong_repl.
-    rewrite <- assoc. rewrite <- assoc. apply strong_repl.
-    specialize(@strong_pair x 0 0). intros.
-    rewrite assoc. rewrite assoc. apply H.
-    transitivity((copair id (update x o 
-    (mult o pair (constant (-1)) (lookup x))) o 
-    (ttrue) o (update x o constant 0))).
-    apply strong_subs. apply strong_repl.
-    apply IMP_IntGeT. simpl. auto.
-    transitivity(id o update x o constant 0).
-    rewrite assoc. apply strong_subs. apply strong_subs.
-    apply strong_coproj_copi1_rwrw. rewrite <- assoc.
-    rewrite id_tgt. apply strong_sym.
-
-    transitivity((copair (update x o 
-    (mult o pair (constant (-1)) (lookup x))) id o 
-    (le o pair (constant 0) (constant 0))) o (update x o constant 0)).
-    rewrite <- assoc. rewrite <- assoc. apply strong_repl.
-    rewrite <- assoc. rewrite <- assoc. apply strong_repl.
-    specialize(@strong_pair x 0 0). intros.
-    rewrite assoc. rewrite assoc. apply H.
-    transitivity((copair (update x o 
-    (mult o pair (constant (-1)) (lookup x))) id o 
-    (ttrue) o (update x o constant 0))).
-    apply strong_subs. apply strong_repl.
-    apply IMP_IntLeT. simpl. auto.
-    transitivity((update x o (mult o pair (constant (-1)) (lookup x)))
-    o update x o constant 0).
-    rewrite assoc. apply strong_subs. apply strong_subs.
-    apply strong_coproj_copi1_rwrw.
-    transitivity(update x o mult o (pair (constant (-1)) (constant 0)) 
-    o update x o constant 0). apply strong_sym.
-    rewrite <- assoc. rewrite <- assoc. rewrite <- assoc. 
-    rewrite <- assoc. rewrite <- assoc. apply strong_repl.
-    rewrite <- assoc. apply strong_repl. apply strong_sym.
-    specialize(@perm_strong_pair x 0 (-1)). intros.
-    rewrite assoc. rewrite assoc. apply H.
-    transitivity(update x o (constant 0) o update x o (constant 0)).
-    apply strong_subs. apply strong_subs. rewrite <- assoc.
-    apply strong_repl. apply IMP_IntMult.
-    specialize(@IMP_ex3 x 0 0). unfold defCommand. unfold defBoolExp. 
-    unfold defArithExp. intros. rewrite <- assoc. apply H. 
- Qed.
-
- Lemma IMP_ex12: forall (x y: Loc), x <> y ->
-       {{x ::= (const 5) ;; y ::= (loc x)}}
-       ==
-       {{y ::= (const 5) ;; x ::= (loc y)}}.
- Proof.
-    intros. unfold defCommand. unfold defBoolExp. 
-    unfold defArithExp. apply strong_sym.
-    transitivity(update x o constant 5 o update y o constant 5).
-    rewrite <- assoc. rewrite <- assoc. rewrite <- assoc.
-    apply strong_repl. remember commutation_lookup_constant.
-    specialize(@commutation_lookup_constant y 5).
-    intros. rewrite assoc. rewrite assoc. apply H0.
-    apply strong_sym. 
-    transitivity(update y o constant 5 o update x o constant 5).
-    rewrite <- assoc. rewrite <- assoc. rewrite <- assoc.
-    apply strong_repl. remember commutation_lookup_constant.
-    specialize(@commutation_lookup_constant x 5).
-    intros. rewrite assoc. rewrite assoc. apply H0.
-    rewrite <- assoc. specialize(@IMP_ex1 y x 5 5).
-    unfold defCommand. unfold defBoolExp. 
-    unfold defArithExp. intros. apply strong_sym.
-    rewrite <- assoc. apply H0. auto.
- Qed.
- 
- Lemma IMP_ex13: forall (x y: Loc), x <> y ->
-       {{x ::= (const 10) ;;
-         y ::= (const 3) ;;
-        IFB ((loc x) >>= (loc y) *** (const 3))
-          THEN (x ::= (loc y)) 
-        ELSE (SKIP) 
-        ENDIF}}
-        ==
-       {{x ::= (const 10) ;;
-         y ::= (const 3) ;;
-        IFB ((loc x) >>= (const 4) *** (loc y)) 
-          THEN (SKIP) 
-        ELSE (x ::= (loc y)) 
-        ENDIF}}.
- Proof.
-    intros. unfold defCommand. unfold defBoolExp. 
-    unfold defArithExp.
-    transitivity(copair (update x o lookup y) id o 
-    ge o pair (lookup x) (mult o pair (constant 3) (constant 3)) o 
-    update y o constant 3  o update x o constant 10).
-    apply strong_sym. repeat rewrite <- assoc.
-    apply strong_repl. repeat rewrite assoc.
-    repeat apply strong_subs. repeat rewrite <- assoc.
-    apply strong_repl. apply strong_unicity. 
-    transitivity(lookup x o update y o constant 3).
-    rewrite assoc. rewrite assoc. apply weak_subs. 
-    apply weak_subs. apply weak_proj_pi1_rorw. auto. 
-    apply weak_sym. repeat rewrite assoc. repeat apply weak_subs.
-    apply weak_proj_pi1_rorw. auto.
-    transitivity( (mult o pair (constant 3) (constant 3)) o 
-    (update y o constant 3)). rewrite assoc. apply strong_subs.
-    apply strong_proj_pi2_rorw. auto. apply strong_sym.
-    transitivity((mult o pair (lookup y) (constant 3)) o 
-    (update y o constant 3)). rewrite assoc. apply strong_subs.
-    apply strong_proj_pi2_rorw. auto. repeat rewrite <- assoc. 
-    apply strong_repl. specialize(@strong_pair y 3 3). intros.
-    repeat rewrite assoc. apply H0.
-    transitivity(copair (update x o lookup y) id o ge o
-    (pair (lookup x) (constant 9)) o update y o
-    constant 3 o update x o constant 10).
-    repeat apply strong_subs. apply strong_repl. apply strong_unicity.
-    transitivity(lookup x). apply weak_proj_pi1_rorw. auto.
-    apply weak_sym. apply weak_proj_pi1_rorw. auto.
-    transitivity(mult o pair (constant 3) (constant 3)).
-    apply strong_proj_pi2_rorw. auto. apply strong_sym.
-    transitivity(constant 9). apply strong_proj_pi2_rorw. auto.
-    apply strong_sym. apply IMP_IntMult.
-    transitivity(copair (update x o lookup y) id o ge o 
-    (pair (lookup x) (constant 9)) o (update x o constant 10) 
-    o (update y o constant 3)). repeat rewrite <- assoc.
-    repeat apply strong_repl. rewrite assoc. specialize(@IMP_ex1 x y 10 3).
-    unfold defCommand. unfold defBoolExp. unfold defArithExp.
-    intros. apply H0. assumption.
-    transitivity((((copair (update x o lookup y) id o ge) o
-    pair (constant 10) (constant 9)) o (update x o constant 10)) o
-    (update y o constant 3)). apply strong_subs. repeat rewrite <- assoc.
-    repeat apply strong_repl. specialize(@strong_pair x 10 9). intros.
-    repeat rewrite assoc. apply H0.
-    transitivity((((copair (update x o lookup y) id o ttrue o 
-    (update x o constant 10)) o (update y o constant 3)))).
-    repeat apply strong_subs. rewrite <- assoc.
-    apply strong_repl. apply IMP_IntGeT. simpl. auto.
-    transitivity((update x o lookup y) o
-    (update x o constant 10) o (update y o constant 3)).
-    repeat apply strong_subs. apply strong_coproj_copi1_rwrw.
-    transitivity(update x o lookup y o update y o constant 3
-    o update x o constant 10). apply strong_sym.
-    repeat rewrite <- assoc. repeat apply strong_repl. rewrite assoc.    
-    specialize(@IMP_ex1 x y 10 3). unfold defCommand.
-    unfold defBoolExp. unfold defArithExp. intros.
-    apply H0. assumption.
-    transitivity(update x o constant 3 o update y o constant 3
-    o update x o constant 10).
-    apply strong_subs. apply strong_subs. repeat rewrite <- assoc.
-    apply strong_repl. specialize(@commutation_lookup_constant y 3).
-    intros. repeat rewrite assoc. apply H0.
-    transitivity(update x o constant 3 o update x o constant 10
-    o update y o constant 3). repeat rewrite <- assoc.
-    repeat apply strong_repl. rewrite assoc.
-    apply strong_sym. rewrite assoc. specialize(@IMP_ex1 y x 3 10).
-    unfold defCommand. unfold defBoolExp. unfold defArithExp.
-    intros. apply H0. auto.
-    transitivity(update x o constant 3 o update y o constant 3).
-    repeat apply strong_subs. rewrite <- assoc.
-    specialize(@IMP_ex3 x 10 3). unfold defCommand. unfold defBoolExp. 
-    unfold defArithExp. intros. apply H0. rewrite <- assoc.
-    (*first program is reduced into following form: x ::= 3 ;; y ::= 3*)
-    apply strong_sym.
-
-    transitivity(copair id (update x o lookup y) o 
-    ge o pair (lookup x) (mult o pair (constant 4) (constant 3)) o 
-    update y o constant 3  o update x o constant 10).
-    apply strong_sym. repeat rewrite <- assoc. apply strong_repl.
-    repeat rewrite assoc. repeat apply strong_subs. 
-    repeat rewrite <- assoc. apply strong_repl. apply strong_unicity. 
-    transitivity(lookup x o update y o constant 3).
-    rewrite assoc. rewrite assoc. repeat apply weak_subs. 
-    apply weak_proj_pi1_rorw. auto. apply weak_sym. 
-    repeat rewrite assoc. repeat apply weak_subs.
-    apply weak_proj_pi1_rorw. auto.
-    transitivity( (mult o pair (constant 4) (constant 3)) o 
-    (update y o constant 3)). rewrite assoc. apply strong_subs.
-    apply strong_proj_pi2_rorw. auto. apply strong_sym.
-    transitivity((mult o pair (constant 4) (lookup y)) o 
-    (update y o constant 3)). rewrite assoc. apply strong_subs.
-    apply strong_proj_pi2_rorw. auto. rewrite <- assoc.
-    rewrite <- assoc. apply strong_repl.
-    specialize(@perm_strong_pair y 3 4). intros. repeat rewrite assoc.
-    apply H0. transitivity(copair id (update x o lookup y) o ge o
-    (pair (lookup x) (constant 12)) o update y o
-    constant 3 o update x o constant 10).
-    repeat apply strong_subs. apply strong_repl. apply strong_unicity.
-    transitivity(lookup x). apply weak_proj_pi1_rorw. auto.
-    apply weak_sym. apply weak_proj_pi1_rorw. auto.
-    transitivity(mult o pair (constant 4) (constant 3)).
-    apply strong_proj_pi2_rorw. auto. apply strong_sym.
-    transitivity(constant 12). apply strong_proj_pi2_rorw. auto.
-    apply strong_sym. apply IMP_IntMult.
-    transitivity(copair id (update x o lookup y) o ge o 
-    (pair (lookup x) (constant 12)) o (update x o constant 10) 
-    o (update y o constant 3)). repeat rewrite <- assoc.
-    repeat apply strong_repl. rewrite assoc. specialize(@IMP_ex1 x y 10 3).
-    unfold defCommand. unfold defBoolExp. unfold defArithExp.
-    intros. apply H0. assumption.
-    transitivity((((copair id (update x o lookup y) o ge) o
-    pair (constant 10) (constant 12)) o (update x o constant 10)) o
-    (update y o constant 3)). apply strong_subs. repeat rewrite <- assoc.
-    repeat apply strong_repl. specialize(@strong_pair x 10 12). intros.
-    rewrite assoc. rewrite assoc. apply H0.
-    transitivity((((copair id (update x o lookup y) o ffalse o 
-    (update x o constant 10)) o (update y o constant 3)))).
-    repeat apply strong_subs. rewrite <- assoc.
-    apply strong_repl. apply IMP_IntGeF. simpl. auto.
-    transitivity((update x o lookup y) o
-    (update x o constant 10) o (update y o constant 3)).
-    repeat apply strong_subs. apply strong_coproj_copi2_rwrw.
-    transitivity(update x o lookup y o update y o constant 3
-    o update x o constant 10). apply strong_sym.
-    repeat rewrite <- assoc. repeat apply strong_repl.
-    rewrite assoc. specialize(@IMP_ex1 x y 10 3). 
-    unfold defCommand. unfold defBoolExp. unfold defArithExp.
-    intros. apply H0. assumption.
-    transitivity(update x o constant 3 o update y o constant 3
-    o update x o constant 10).
-    apply strong_subs. apply strong_subs. repeat rewrite <- assoc.
-    apply strong_repl. specialize(@commutation_lookup_constant y 3).
-    intros. repeat rewrite assoc. apply H0.
-    transitivity(update x o constant 3 o update x o constant 10
-    o update y o constant 3). repeat rewrite <- assoc.
-    repeat apply strong_repl. rewrite assoc. apply strong_sym.
-    rewrite assoc. specialize(@IMP_ex1 y x 3 10).
-    unfold defCommand. unfold defBoolExp. unfold defArithExp.
-    intros. apply H0. auto.
-    transitivity(update x o constant 3 o update y o constant 3).
-    repeat apply strong_subs. rewrite <- assoc.
-    specialize(@IMP_ex3 x 10 3). unfold defCommand. unfold defBoolExp. 
-    unfold defArithExp. intros. apply H0. rewrite <- assoc.
-    (*second program is reduced into following form: x ::= 3 ;; y ::= 3*)
-    apply strong_refl.
+      intros. simpl. induction b. rewrite copair_true; apply strong_refl.
+      setoid_rewrite copair_false; apply strong_refl.
  Qed. 
 
- Lemma IMP_ex14: forall (x: Loc),
-       {{x ::= (const 10) ;;
-        IFB ((loc x) >>= (const 0)) 
-          THEN (IFB ((loc x) === (const 10))
-                  THEN (x ::= (const 20))
-                ELSE (SKIP)
-                ENDIF)
-        ELSE (x ::= (const 30)) 
+ Lemma IMP_condEx2: forall (b: bool) (f g h: Command),
+       {{IFB const b
+          THEN (IFB const b THEN f ELSE g ENDIF)
+        ELSE h
         ENDIF}}
-        ==
-       {{x ::= (const 20)}}.
+      ==
+      {{IFB const b
+          THEN f
+        ELSE h
+        ENDIF}}.
  Proof.
-    intros. unfold defCommand. unfold defBoolExp. 
-    unfold defArithExp.
-    transitivity((copair (copair (update x o constant 20) id o 
-    (eq o pair (lookup x) (constant 10)))
-    (update x o constant 30) o (ge o pair (constant 10) (constant 0))) o 
-    (update x o constant 10)).
-    repeat rewrite <- assoc. apply strong_repl. repeat rewrite <- assoc.
-    apply strong_repl. specialize(@strong_pair x 10 0). intros.
-    repeat rewrite assoc. apply H.
-    transitivity((copair (copair (update x o constant 20) id o
-    (eq o pair (lookup x) (constant 10))) (update x o constant 30) 
-    o (ttrue) o (update x o constant 10))).
-    repeat rewrite <- assoc. apply strong_repl. apply strong_subs.
-    apply IMP_IntGeT. simpl. auto.
-    transitivity((copair (update x o constant 20) id o 
-    (eq o pair (lookup x) (constant 10))) o (update x o constant 10)).
-    repeat rewrite assoc. repeat apply strong_subs. 
-    apply strong_coproj_copi1_rwrw.
-    transitivity((copair (update x o constant 20) id o 
-    (eq o pair (constant 10) (constant 10))) o
-    (update x o constant 10)). repeat rewrite <- assoc.
-    apply strong_repl. repeat rewrite <- assoc. apply strong_repl.
-    specialize(@strong_pair x 10 10). intros. repeat rewrite assoc.
-    apply H. 
-    transitivity((copair (update x o constant 20) id o 
-    (ttrue) o (update x o constant 10))). apply strong_subs.
-    apply strong_repl. apply IMP_IntEqT. simpl. auto.
-    transitivity((update x o constant 20) o (update x o constant 10)).
-    apply strong_subs. apply strong_coproj_copi1_rwrw.
-    specialize(@IMP_ex3 x 10 20). unfold defCommand. unfold defBoolExp. 
-    unfold defArithExp. intros. apply H.    
+      intros. simpl. induction b. rewrite copair_true. setoid_rewrite copair_true.
+      apply strong_refl. setoid_rewrite copair_false; apply strong_refl.
+ Qed. 
+
+ Lemma IMP_ex6lbdyT: forall (x : Loc) (p q r: Z), Is_true(chklt (q, r)) -> (*(bool_to_prop (chklt (q, r))) ->*)
+	{{x ::= const q ;;
+	  WHILE (loc x << const r)
+	    DO x ::= (loc x +++ const p)
+	  ENDWHILE}}
+	==
+	{{x ::= const (q+p) ;;
+	  WHILE (loc x << const r)
+	    DO x ::= (loc x +++ const p)
+	  ENDWHILE}}.
+ Proof.
+    intros. simpl. do 2 setoid_rewrite assoc at 2. setoid_rewrite <- assoc at 1. 
+     rewrite commutation_lookup_constant_update. do 2 setoid_rewrite <- assoc at 1.
+     do 3 setoid_rewrite assoc at 6. rewrite IMP_IntLtT by assumption. do 2 rewrite assoc.
+     rewrite strong_coproj_copi1_rwrw. do 4 rewrite <- assoc.
+     rewrite commutation_lookup_constant_update. do 3 rewrite assoc. 
+     setoid_rewrite <- assoc at 2. rewrite IMP_IntAdd. setoid_rewrite <- assoc at 2.
+     setoid_rewrite <- assoc at 1. rewrite (@IMP_ex3 x q (add(q,p))). simpl.
+     setoid_rewrite (@IMP_Loop (passbool o (tpure chklt o pair (lookup x) (constant r)))
+       (update x o (tpure add o pair (lookup x) (constant p)))) at 1. reflexivity.
+ Qed. 
+
+ Lemma IMP_ex6lbdyF: forall (x : Loc) (p q r: Z), Is_true(chkge (q, r)) ->
+	{{x ::= const q ;;
+	  WHILE (loc x << const r)
+	    DO x ::= (loc x +++ const p)
+	  ENDWHILE}}
+    ==
+        {{x ::= const q}}.
+ Proof.
+     intros. simpl. do 2 setoid_rewrite assoc at 2. setoid_rewrite <- assoc at 1. 
+     rewrite commutation_lookup_constant_update. do 2 setoid_rewrite <- assoc at 1.
+     do 3 setoid_rewrite assoc at 6. rewrite IMP_IntLtF by assumption. do 2 rewrite assoc.
+     rewrite strong_coproj_copi2_rwrw. rewrite id_tgt. reflexivity.
  Qed.
 
  Lemma IMP_ex15: forall (x: Loc),
-	{{x ::= (const 2) ;;
-	  WHILE ((loc x) << (const 11))
-	    DO (x ::= ((loc x) +++ (const 4)))
+	{{x ::= const 2 ;;
+	  WHILE (loc x << const 11)
+	    DO x ::= (loc x +++ const 4)
 	  ENDWHILE}}
 	==
-	{{x ::= (const 14)}}.
+	{{x ::= const 14}}.
  Proof.
-    intros. unfold defCommand. unfold defBoolExp. 
-    unfold defArithExp. 
-    transitivity((copair (loopdec o (update x o 
-    (plus o pair (lookup x) (constant 4)))) id o 
-    (lt o pair (constant 2) (constant 11))) o (update x o constant 2)).
-    repeat rewrite <- assoc. apply strong_repl. repeat rewrite <- assoc.
-    apply strong_repl. specialize(@strong_pair x 2 11). intros.
-    repeat rewrite assoc. apply H. 
-    transitivity((copair (loopdec o (update x o 
-    (plus o pair (lookup x) (constant 4)))) id o 
-    (ttrue) o (update x o constant 2))).
-    apply strong_subs. apply strong_repl. apply IMP_IntLtT. simpl. auto.
-    transitivity(loopdec o (update x o (plus o pair (lookup x) (constant 4))) o 
-    update x o constant 2). rewrite assoc. repeat apply strong_subs.
-    apply strong_coproj_copi1_rwrw. rewrite <- assoc.
-    transitivity(loopdec o update x o plus o (pair (constant 2) (constant 4)) o
-    update x o constant 2). apply strong_sym. repeat rewrite <- assoc. 
-    apply strong_repl. rewrite <- assoc. apply strong_repl. rewrite <- assoc. 
-    apply strong_repl. specialize(@strong_pair x 2 4). intros. apply strong_sym.
-    repeat rewrite assoc. apply H. 
-    transitivity(loopdec o update x o constant 6 o update x o constant 2).
-    repeat apply strong_subs. rewrite <- assoc. apply strong_repl.
-    apply IMP_IntAdd.
-    transitivity(loopdec o update x o constant 6).
-    repeat rewrite <- assoc. apply strong_repl. rewrite assoc.
-    specialize(@IMP_ex3 x 2 6). unfold defCommand. unfold defBoolExp. 
-    unfold defArithExp. intros. apply H. 
-
-    transitivity((copair (loopdec o (update x o 
-    (plus o pair (lookup x) (constant 4)))) id o 
-    (lt o pair (lookup x) (constant 11))) o (update x o constant 6)).
-
-    remember IMP_Loop.
-
-    specialize(@IMP_Loop (lt o pair (lookup x) (constant 11)) 
-    (update x o (plus o pair (lookup x) (constant 4))) (loopdec)).
-    intros. rewrite assoc. repeat apply strong_subs. apply H.
-
-    transitivity((copair (loopdec o (update x o 
-    (plus o pair (lookup x) (constant 4)))) id o 
-    (lt o pair (constant 6) (constant 11))) o (update x o constant 6)).
-    repeat rewrite <- assoc. apply strong_repl. repeat rewrite <- assoc.
-    apply strong_repl. specialize(@strong_pair x 6 11). intros.
-    repeat rewrite assoc. apply H. 
-    transitivity((copair (loopdec o (update x o 
-    (plus o pair (lookup x) (constant 4)))) id o 
-    (ttrue) o (update x o constant 6))).
-    apply strong_subs. apply strong_repl. apply IMP_IntLtT. simpl. auto.
-    transitivity(loopdec o (update x o (plus o pair (lookup x) (constant 4))) o 
-    update x o constant 6). rewrite assoc. repeat apply strong_subs.
-    apply strong_coproj_copi1_rwrw. rewrite <- assoc.
-    transitivity(loopdec o update x o plus o (pair (constant 6) (constant 4)) o
-    update x o constant 6). apply strong_sym. repeat rewrite <- assoc. 
-    apply strong_repl. rewrite <- assoc. apply strong_repl. rewrite <- assoc. 
-    apply strong_repl. specialize(@strong_pair x 6 4). intros. apply strong_sym.
-    repeat rewrite assoc. apply H. 
-    transitivity(loopdec o update x o constant 10 o update x o constant 6).
-    repeat apply strong_subs. rewrite <- assoc. apply strong_repl.
-    apply IMP_IntAdd.
-    transitivity(loopdec o update x o constant 10).
-    repeat rewrite <- assoc. apply strong_repl. rewrite assoc.
-    specialize(@IMP_ex3 x 6 10). unfold defCommand. unfold defBoolExp. 
-    unfold defArithExp. intros. apply H. 
-
-    transitivity((copair (loopdec o (update x o 
-    (plus o pair (lookup x) (constant 4)))) id o 
-    (lt o pair (lookup x) (constant 11))) o (update x o constant 10)).
-
-    remember IMP_Loop.
-
-    specialize(@IMP_Loop (lt o pair (lookup x) (constant 11)) 
-    (update x o (plus o pair (lookup x) (constant 4))) (loopdec)).
-    intros. rewrite assoc. repeat apply strong_subs. apply H.
-
-    transitivity((copair (loopdec o (update x o 
-    (plus o pair (lookup x) (constant 4)))) id o 
-    (lt o pair (constant 10) (constant 11))) o (update x o constant 10)).
-    repeat rewrite <- assoc. apply strong_repl. repeat rewrite <- assoc.
-    apply strong_repl. specialize(@strong_pair x 10 11). intros.
-    repeat rewrite assoc. apply H. 
-    transitivity((copair (loopdec o (update x o 
-    (plus o pair (lookup x) (constant 4)))) id o 
-    (ttrue) o (update x o constant 10))).
-    apply strong_subs. apply strong_repl. apply IMP_IntLtT. simpl. auto.
-    transitivity(loopdec o (update x o (plus o pair (lookup x) (constant 4))) o 
-    update x o constant 10). rewrite assoc. repeat apply strong_subs.
-    apply strong_coproj_copi1_rwrw. rewrite <- assoc.
-    transitivity(loopdec o update x o plus o (pair (constant 10) (constant 4)) o
-    update x o constant 10). apply strong_sym. repeat rewrite <- assoc. 
-    apply strong_repl. rewrite <- assoc. apply strong_repl. rewrite <- assoc. 
-    apply strong_repl. specialize(@strong_pair x 10 4). intros. apply strong_sym.
-    repeat rewrite assoc. apply H. 
-    transitivity(loopdec o update x o constant 14 o update x o constant 10).
-    repeat apply strong_subs. rewrite <- assoc. apply strong_repl.
-    apply IMP_IntAdd.
-    transitivity(loopdec o update x o constant 14).
-    repeat rewrite <- assoc. apply strong_repl. rewrite assoc.
-    specialize(@IMP_ex3 x 10 14). unfold defCommand. unfold defBoolExp. 
-    unfold defArithExp. intros. apply H. 
-
-    transitivity((copair (loopdec o (update x o 
-    (plus o pair (lookup x) (constant 4)))) id o 
-    (lt o pair (lookup x) (constant 11))) o (update x o constant 14)).
-
-    remember IMP_Loop.
-
-    specialize(@IMP_Loop (lt o pair (lookup x) (constant 11)) 
-    (update x o (plus o pair (lookup x) (constant 4))) (loopdec)).
-    intros. rewrite assoc. repeat apply strong_subs. apply H.
-
-    transitivity((copair (loopdec o (update x o 
-    (plus o pair (lookup x) (constant 4)))) id o 
-    (lt o pair (constant 14) (constant 11))) o (update x o constant 14)).
-    repeat rewrite <- assoc. apply strong_repl. repeat rewrite <- assoc.
-    apply strong_repl. specialize(@strong_pair x 14 11). intros.
-    repeat rewrite assoc. apply H. 
-    transitivity((copair (loopdec o (update x o 
-    (plus o pair (lookup x) (constant 4)))) id o 
-    (ffalse) o (update x o constant 14))).
-    apply strong_subs. apply strong_repl. apply IMP_IntLtF. simpl. auto.
-    transitivity(id o (update x o constant 14)). apply strong_subs.
-    apply strong_coproj_copi2_rwrw. rewrite id_tgt. apply strong_refl.
+     intros; simpl.
+     rewrite(@IMP_ex6lbdyT x 4 2 11) by constructor; simpl.
+     rewrite(@IMP_ex6lbdyT x 4 6 11) by constructor; simpl.
+     rewrite(@IMP_ex6lbdyT x 4 10 11) by constructor; simpl.
+     rewrite(@IMP_ex6lbdyF x 4 14 11) by constructor; reflexivity.
  Qed.
 
- Lemma IMP_ex16: forall (x: Loc),
-       {{x ::= (const 50) ;;
-         IFB ((loc x) << (const 70) &&& (loc x) >> (const 40))
-           THEN (x ::= (const 10))
-         ELSE (SKIP)
-         ENDIF}}
-       ==
-       {{x ::= (const 10)}}.
- Proof.
-    intros. unfold defCommand. unfold defBoolExp. 
-    unfold defArithExp. 
-    transitivity((copair (update x o constant 10) id o 
-    (andB o pair (lt o pair (constant 50) (constant 70))
-    (gt o pair (constant 50) (constant 40)))) o (update x o constant 50)).
-    repeat rewrite <- assoc. apply strong_repl. repeat rewrite <- assoc.
-    apply strong_repl. apply strong_unicity.
-    transitivity(lt o (pair (lookup x) (constant 70)) o
-    (update x o constant 50)). rewrite assoc.
-    apply weak_subs. apply weak_proj_pi1_rorw. auto.
-    apply weak_sym.
-    transitivity(lt o (pair (constant 50) (constant 70)) o
-    (update x o constant 50)). rewrite assoc. apply weak_subs.
-    apply weak_proj_pi1_rorw. auto. apply strong_to_weak. apply strong_sym.
-    specialize(@strong_pair x 50 70). intros.
-    repeat rewrite <- assoc. apply strong_repl. repeat rewrite assoc. apply H.
-    
-    transitivity((gt o pair (lookup x) (constant 40)) o (update x o constant 50)).
-    rewrite assoc. apply strong_subs. apply strong_proj_pi2_rorw. auto.
-    transitivity((gt o pair (constant 50) (constant 40)) o (update x o constant 50)).
-    specialize(@strong_pair x 50 40). intros.
-    repeat rewrite <- assoc. apply strong_repl. repeat rewrite assoc. apply H.
-    apply strong_sym. rewrite assoc. apply strong_subs.
-    apply strong_proj_pi2_rorw. auto.
-
-    transitivity((copair (update x o constant 10) id o (andB
-    o (pair ttrue ttrue) o (update x o constant 50)))).
-    rewrite <- assoc. apply strong_repl. apply strong_subs.
-    apply strong_repl. apply strong_unicity.
-    transitivity(lt o pair (constant 50) (constant 70)).
-    apply weak_proj_pi1_rorw. auto. transitivity(ttrue).
-    apply strong_to_weak. apply IMP_IntLtT. simpl. auto.
-    apply weak_sym. apply weak_proj_pi1_rorw. apply is_pure_ro. apply is_ttrue.
-    transitivity(gt o pair (constant 50) (constant 40)).
-    apply strong_proj_pi2_rorw. auto. transitivity(ttrue).
-    apply IMP_IntGtT. simpl. auto. apply strong_sym.
-    apply strong_proj_pi2_rorw. apply is_pure_ro. apply is_ttrue.
-    
-    transitivity(copair (update x o constant 10) id o 
-    ttrue o (update x o constant 50)).
-    apply strong_sym. rewrite <- assoc. apply strong_repl.
-    apply strong_subs. apply strong_sym. apply IMP_IntAndT.
-    apply one_weak_to_strong. auto. apply is_comp. auto.
-    apply is_pair. repeat apply is_pure_ro; apply is_ttrue.
-    repeat apply is_pure_ro; apply is_ttrue.
-    repeat apply is_pure_ro; apply is_ttrue. apply weak_proj_pi1_rorw. 
-    repeat apply is_pure_ro; apply is_ttrue.
-    apply strong_proj_pi2_rorw. repeat apply is_pure_ro; apply is_ttrue.
-    transitivity((update x o constant 10) o (update x o constant 50)).
-    apply strong_subs. apply strong_coproj_copi1_rwrw.
-   
-    specialize(@IMP_ex3 x 50 10). unfold defCommand. unfold defBoolExp. 
-    unfold defArithExp. intros. apply H.    
- Qed.
-
- Lemma IMP_ex17: forall (x: Loc), forall (p: Z),
-         {{ IFB ((const p) << (const 0))
-           THEN (x ::= (const 100))
-         ELSE (x ::= (const p))
-         ENDIF}}
-         ==
-         {{ IFB ((const p) >>= (const 0))
-           THEN (x ::= (const p))
-         ELSE (x ::= (const 100))
-         ENDIF}}.
- Proof.
-    intros. unfold defCommand. unfold defBoolExp. 
-    unfold defArithExp. induction p.
-    transitivity(copair (update x o constant 100) (update x o constant 0) o ffalse).
-    apply strong_repl. apply IMP_IntLtF. simpl. auto.
-    transitivity(update x o constant 0).
-    apply strong_coproj_copi2_rwrw. apply strong_sym.
-    transitivity(copair (update x o constant 0) (update x o constant 100) o ttrue).
-    apply strong_repl. apply IMP_IntGeT. simpl. auto.
-    transitivity(update x o constant 0).
-    apply strong_coproj_copi1_rwrw. apply strong_refl.
-    transitivity(copair (update x o constant 100) (update x o constant (Zpos p)) o ffalse).
-    apply strong_repl. apply IMP_IntLtF. simpl. auto.
-    transitivity(update x o constant (Zpos p)). apply strong_coproj_copi2_rwrw.
-    apply strong_sym.
-    transitivity(copair (update x o constant (Zpos p)) (update x o constant 100) o ttrue).
-    apply strong_repl. apply IMP_IntGeT. simpl. auto.
-    transitivity(update x o constant (Zpos p)). apply strong_coproj_copi1_rwrw.
-    apply strong_refl.
-    transitivity(copair (update x o constant 100) (update x o constant (Zneg p)) o ttrue).
-    apply strong_repl. apply IMP_IntLtT. simpl. auto.
-    transitivity(update x o constant 100). apply strong_coproj_copi1_rwrw.
-    apply strong_sym.
-    transitivity(copair (update x o constant (Zneg p)) (update x o constant 100) o ffalse).
-    apply strong_repl. apply IMP_IntGeF. simpl. auto.
-    transitivity(update x o constant 100). apply strong_coproj_copi2_rwrw.
-    apply strong_refl.
- Qed.
 
 End Make.
+
+   
