Memory.v
@@ -1,7 +1,7 @@
 (**************************************************************************)
-(*  This is part of IMP-STATES, it is distributed under the terms of the  *)
-(*              GNU Lesser General Public License version 3               *)
-(*                  (see file LICENSE for more details)                   *)
+(*  This is part of STATES, it is distributed under the terms of the      *)
+(*         GNU Lesser General Public License version 3                    *)
+(*              (see file LICENSE for more details)                       *)
 (*                                                                        *)
 (*       Copyright 2014: Jean-Guillaume Dumas, Dominique Duval            *)
 (*			 Burak Ekici, Damien Pous.                        *)
@@ -11,19 +11,11 @@ Require Import Relations Morphisms.
 Require Import Program.
 Require Import Le Gt Minus Bool Setoid.
 Set Implicit Arguments.
-Require Import ZArith.
-Open Scope Z_scope.
 
 Module Type T.
  Parameter Loc: Type.
  Parameter Val: Loc -> Type.
  Parameter Loc_dec: forall i j: Loc, {i=j}+{i<>j}.
-
- Parameter EName: Type.
- Parameter EVal: EName -> Type.
- Parameter Exc_dec: forall i j: EName, {i=j}+{i<>j}.
-
- Parameter empty_set: Set.
 
 End T.
 
