Proofs.v
@@ -1,0 +1,165 @@
+(**************************************************************************)
+(*  This is part of STATES, it is distributed under the terms of the      *)
+(*         GNU Lesser General Public License version 3                    *)
+(*              (see file LICENSE for more details)                       *)
+(*                                                                        *)
+(*       Copyright 2014: Jean-Guillaume Dumas, Dominique Duval            *)
+(*			 Burak Ekici, Damien Pous.                        *)
+(**************************************************************************)
+
+Require Import Relations Morphisms.
+Require Import Program.
+Require Memory Terms Decorations Axioms Derived_Terms Derived_Pairs
+        Derived_Products Derived_Rules.
+Set Implicit Arguments.
+Require Import ZArith.
+Open Scope Z_scope.
+
+
+Module Make(Import M: Memory.T).
+  Module Export ProofsExp := Derived_Rules.Make(M). 
+
+(* --- Main Proofs --- *)
+
+ Theorem annihilation_update_lookup: forall i: Loc, 
+         update i o lookup i == id.
+         (* Prop: 2.1: All Cases *)
+ Proof.
+     intro. remember observation. apply observation. intro k.
+     destruct (Loc_dec i k). rewrite <- e.
+     (*Case k = i*)
+     rewrite assoc. setoid_rewrite -> id_src. setoid_rewrite <- id_tgt at 6.
+     apply wsc. apply axiom_1. apply strong_refl.
+     (*Case k <> i*)
+     rewrite assoc. remember wsc. rewrite axiom_2; try decorate.
+     apply strong_to_weak. rewrite <- assoc. apply sc. apply strong_refl.
+     apply E_1_4; decorate.
+ Qed.
+
+ Theorem interaction_lookup_lookup: forall i,
+         lookup i o forget o lookup i == lookup i.
+         (* Prop: 2.2: All Cases: Simplified Version *)
+ Proof.
+     intros. setoid_rewrite <- id_src at 6. rewrite <- assoc. apply sc.
+     apply strong_refl. apply E_1_4; decorate.
+ Qed.
+
+ Theorem interaction_update_lookup: forall i: Loc,
+         lookup i o update i ~~ id. (* Prop: 2.4: All Cases *)
+ Proof. intros. apply axiom_1. Qed.
+
+ Theorem commutation_lookup_lookup: forall i j: Loc, i<>j ->
+         (prod id (lookup j)) o (inv_pi1 o lookup i)
+         == 
+         permut o ((prod id (lookup i)) o (inv_pi1 o lookup j)). 
+         (* Prop: 2.5: All Cases *)
+ Proof.
+    intros. remember strong_unicity.
+    specialize (@strong_unicity _ _ _
+    (prod id (lookup j) o (inv_pi1 o lookup i)) 
+    ((permut) o ((prod id (lookup i)) o (inv_pi1 o lookup j)))).
+    intros. apply H0.
+    (*Case pi1*)
+    setoid_rewrite assoc at 1. remember wsc.
+    rewrite strong_proj_pi1_purero_rect; try decorate. rewrite id_tgt.
+    rewrite assoc. unfold inv_pi1. rewrite strong_proj_pi1_purero; try decorate.
+    rewrite id_tgt. apply weak_sym.
+    (*Step 2*)
+    rewrite assoc. apply strong_to_weak. remember sc.
+    rewrite strong_pi1_permut__pi2. rewrite assoc. 
+    rewrite strong_proj_pi2_purero_rect; try decorate. rewrite assoc.
+    setoid_rewrite <- assoc at 2. rewrite strong_proj_pi2_purero; try decorate.
+    rewrite <- assoc. rewrite E_1_4; try decorate. rewrite id_src. apply strong_refl.
+    (*Case pi2*)
+    rewrite assoc. remember sc. rewrite strong_proj_pi2_purero_rect; try decorate.
+    rewrite assoc. setoid_rewrite <- assoc at 2. rewrite strong_pi2_inv_pi1__unit.
+    rewrite <- assoc. rewrite E_1_4; try decorate. rewrite id_src. apply strong_sym.
+    (*Step 2*)
+    rewrite assoc. rewrite strong_pi2_permut__pi1. rewrite assoc.
+    rewrite strong_proj_pi1_purero_rect; try decorate. rewrite id_tgt.
+    rewrite assoc. unfold inv_pi1. rewrite strong_proj_pi1_purero; try decorate.
+    rewrite id_tgt. apply strong_refl.
+ Qed.
+
+ Theorem commutation_lookup_constant: forall i: Loc, forall c: Z, 
+         (lookup i o (update i o (constant c)))
+         == 
+         (constant c) o update i o (constant c).
+         (*Prop 2.8: All Cases*)
+ Proof.
+     intros. remember comp_final_unique. specialize (@comp_final_unique _ _
+     (lookup i o (update i o (constant c))) 
+     ((constant c) o (update i o (constant c)))).
+     intros. setoid_rewrite <- assoc at 1. apply H.
+     (* Case 1: <> o f == <> o g *)
+     rewrite assoc. specialize (@E_1_4 _ (lookup i)). intros. remember sc. 
+     rewrite H0; try decorate. rewrite id_tgt. apply strong_sym. rewrite assoc.
+     specialize (@E_0_4 _ (constant c)).  intros. rewrite H1; try decorate. 
+     rewrite id_tgt. apply strong_refl. 
+     (* Case 2: f ~ g *)
+     rewrite assoc. remember wsc. rewrite axiom_1. rewrite id_tgt.
+     rewrite <- id_src at 1. apply wrc; try decorate. apply weak_final_unique.
+ Qed.
+
+ Lemma commutation_lookup_constant_update: forall (m: Loc) (p q: Z),
+      (pair (lookup m) (constant q)) o (update m o constant p)
+      ==
+      (pair (constant p) (constant q)) o (update m o constant p).
+ Proof.
+      intros. apply strong_unicity. repeat rewrite assoc. remember wrc. 
+      rewrite weak_proj_pi1_rorw;  try decorate. rewrite axiom_1.
+      rewrite id_tgt. apply weak_sym.
+      repeat rewrite assoc. rewrite weak_proj_pi1_rorw;  try decorate.
+      setoid_rewrite <- id_src at 6. rewrite <- assoc.
+      apply wrc; (solve[decorate] || idtac). apply weak_final_unique.
+      repeat rewrite assoc. remember sc. 
+      rewrite strong_proj_pi2_rorw;  try decorate. apply strong_sym.
+      rewrite strong_proj_pi2_rorw;  try decorate. apply strong_refl.     
+ Qed.
+
+ Lemma commutation_constant_lookup_update: forall (m: Loc) (p q: Z),
+      (pair (constant q) (lookup m)) o (update m o constant p)
+      ==
+      (pair (constant q) (constant p)) o (update m o constant p).
+ Proof.
+      intros. apply strong_unicity. repeat rewrite assoc. remember wrc.
+      rewrite weak_proj_pi1_rorw;  try decorate. apply weak_sym.
+      rewrite weak_proj_pi1_rorw;  try decorate. apply weak_refl.
+      repeat rewrite assoc. remember sc.
+      rewrite strong_proj_pi2_rorw;  try decorate.  
+      specialize(@commutation_lookup_constant m p). intros.
+      rewrite <- assoc. rewrite H. apply strong_sym.
+      rewrite strong_proj_pi2_rorw;  try decorate. apply strong_refl.
+ Qed. 
+
+Lemma commutation_update_update: forall {x y: Loc}, forall (n m: Z), x<>y -> 
+	(update y o constant m) o (update x o constant n) == 
+        (update x o constant n) o (update y o constant m).
+ Proof.
+    intros. apply observation. intros.
+    (* i = y *)
+    destruct (Loc_dec i y). rewrite e. repeat rewrite assoc. rewrite axiom_1. 
+    intros. apply weak_sym. rewrite  axiom_2; try decorate. specialize(@E_0_4 _ (constant n)). 
+    intros. setoid_rewrite <- assoc at 3. rewrite H0; try decorate.
+    setoid_rewrite id_src. rewrite axiom_1. rewrite id_tgt. apply weak_sym.
+    specialize(@weak_final_unique _ (update x o (constant n)) (@id unit)).
+    intros. rewrite <- assoc. rewrite H1. rewrite id_src. apply weak_refl.
+    (* i = x *)
+    destruct (Loc_dec i x). rewrite e. repeat rewrite assoc. rewrite  axiom_2.
+    specialize(@E_0_4 _ (constant m)). intros. setoid_rewrite <- assoc at 3.
+    rewrite H0; try decorate. setoid_rewrite id_src. rewrite axiom_1. rewrite id_tgt.
+    setoid_rewrite <- id_src at 1. rewrite <- assoc. apply wrc; try decorate.
+    apply weak_final_unique. auto.
+    (* i <> x and i <> y *)
+    repeat rewrite assoc. rewrite axiom_2; (auto || idtac). specialize(@E_0_4 _ (constant m)).
+    intros. setoid_rewrite <- assoc at 3. rewrite H0; (solve[decorate] || idtac).
+    rewrite id_src. rewrite axiom_2; (auto || idtac). rewrite <- assoc. apply weak_sym.
+    remember E_0_4. specialize(@E_0_4 _ (constant n)). intros.
+    remember wsc. rewrite H1 at 1; try decorate. rewrite id_src. rewrite assoc. 
+    rewrite axiom_2; auto. repeat rewrite <- assoc. apply strong_to_weak. apply sc.
+    apply strong_refl. apply one_weak_to_strong; try decorate. apply weak_final_unique.
+ Qed.
+
+(* -------------------- End of Main Proofs -------------------- *)
+
+End Make.
